src/matroid.lean
@@ -1,382 +1,75 @@
 /-
-Matroids, after Chapter 1 of Oxley, Matroid Theory, 1992.
+Copyright (c) 2019-2020 Bryan Gin-ge Chen. All rights reserved.
+Released under Apache 2.0 license as described in the file LICENSE.
+Authors: Bryan Gin-ge Chen (with help from Mario Carneiro, Chris Hughes,
+Kenny Lau and others in the Leanprover Zulip chat room).
 -/
-import data.finset tactic.wlog data.equiv.list tactic.find
+import for_mathlib
 
-variables {α : Type*} {β : Type*}
-/- For mathlib?: -/
-/- Everything from here to inter_of_subsete is by Mario Carneiro:
-https://gist.github.com/digama0/edc2a9fe4d468c3921c87650eea5b77a -/
-namespace multiset
-open nat
+/-!
+Matroids, after Chapter 1 of Oxley, Matroid Theory, 1992.
 
-@[simp] theorem card_filter_map_le {α β} {f : α → option β}
-  (s : multiset α) : card (filter_map f s) ≤ card s :=
-multiset.induction_on s (nat.zero_le _) begin
-  intros a s IH,
-  cases h : f a,
-  { rw [filter_map_cons_none _ _ h, card_cons],
-    exact le_succ_of_le IH, },
-  { rw [filter_map_cons_some _ _ _ h, card_cons, card_cons],
-    exact succ_le_succ IH, },
-end
+We begin with the two axiomatizations of matroids defined in Whitney's 1935 paper:
+- matroids from independent sets
+- matroids from circuits
 
-end multiset
+Everything in this file is under the `matroid` namespace, so we have named the two
+structures `of_indep` and `of_circuits`, respectively, so that their fully-qualified
+names are `matroid.of_indep` and `matroid.of_circuits`.
 
-namespace finset
-open nat
-
-def filter_map {α β} [decidable_eq β] (f : α → option β) (s : finset α) : finset β :=
-(s.1.filter_map f).to_finset
-
-@[simp] theorem filter_map_empty {α β} [decidable_eq β] (f : α → option β) :
-  filter_map f ∅ = ∅ := rfl
-
-@[simp] theorem mem_filter_map {α β} [decidable_eq β] {f : α → option β} {s : finset α}
-  {b : β} : b ∈ s.filter_map f ↔ ∃ a ∈ s, b ∈ f a :=
-by { simp only [filter_map, exists_prop, multiset.mem_filter_map, multiset.mem_to_finset], refl, }
-
-theorem card_filter_map_le {α β} [decidable_eq β] {f : α → option β} {s : finset α} :
-  card (s.filter_map f) ≤ card s :=
-le_trans (multiset.card_le_of_le $ multiset.erase_dup_le _)
-  (multiset.card_filter_map_le _)
-
-theorem filter_map_insert_none {α β} [decidable_eq α] [decidable_eq β]
-  (f : α → option β) {a : α} {s : finset α} (hf : f a = none) :
-  filter_map f (insert a s) = filter_map f s :=
-begin
-  by_cases a ∈ s,
-  { rw insert_eq_of_mem h },
-  { simp only [filter_map, multiset.ndinsert_of_not_mem h,
-      multiset.filter_map_cons_none _ _ hf, finset.insert_val], },
-end
-
-theorem filter_map_insert_some {α β} [decidable_eq α] [decidable_eq β]
-  (f : α → option β) {a : α} {s : finset α} {b} (hf : f a = some b) :
-  filter_map f (insert a s) = insert b (filter_map f s) :=
-begin
-  by_cases a ∈ s,
-  { rw [insert_eq_of_mem h, insert_eq_of_mem],
-    exact mem_filter_map.2 ⟨_, h, hf⟩, },
-  { simp only [filter_map, multiset.ndinsert_of_not_mem h,
-      multiset.filter_map_cons_some _ _ _ hf, multiset.to_finset_cons, finset.insert_val], },
-end
-
-theorem mem_of_card_filter_map {α β} [decidable_eq α] [decidable_eq β] {f : α → option β} {s : finset α}
-  (h : card (s.filter_map f) = card s) {a} (ha : a ∈ s) : ∃ b, b ∈ f a :=
-begin
-  cases h' : f a with b, swap, {exact ⟨b, rfl⟩},
-  refine (not_succ_le_self (card (erase s a)) (_ : _ + 1 ≤ _)).elim,
-  rw [← insert_erase ha, filter_map_insert_none f h',
-    card_insert_of_not_mem (not_mem_erase _ _)] at h, rw ← h,
-  apply card_filter_map_le,
-end
-
-theorem inj_of_card_filter_map {α β} [decidable_eq α] [decidable_eq β] {f : α → option β} {s : finset α}
-  (H : card (s.filter_map f) = card s) {a a'} (ha : a ∈ s) (ha' : a' ∈ s)
-    {b} (h1 : b ∈ f a) (h2 : b ∈ f a') : a = a' :=
-begin
-  by_contra h,
-  rw [← insert_erase ha', filter_map_insert_some f h2,
-    card_insert_of_not_mem (not_mem_erase _ _), insert_eq_of_mem] at H,
-  { refine (not_succ_le_self (card (erase s a')) (_ : _ + 1 ≤ _)).elim,
-    rw ← H, apply card_filter_map_le },
-  { exact mem_filter_map.2 ⟨_, mem_erase.2 ⟨h, ha⟩, h1⟩ }
-end
-
-theorem exists_subset_filter_map_eq
-  {α β} [decidable_eq α] [decidable_eq β] (f : α → option β) (s : finset α) :
-  ∃ t ⊆ s, s.filter_map f = filter_map f t ∧ card (t.filter_map f) = card t :=
-begin
-  refine finset.induction_on s ⟨∅, by { simp only [finset.empty_subset, finset.card_empty,
-    exists_prop_of_true, finset.filter_map_empty, and_self, eq_self_iff_true] }⟩ _,
-  rintro a s as ⟨t, ss, st, ct⟩,
-  cases h : f a with b,
-  { refine ⟨t, subset.trans ss (subset_insert _ _), _, ct⟩,
-    simpa only [filter_map_insert_none f h] },
-  simp only [filter_map_insert_some f h],
-  by_cases h' : b ∈ filter_map f s,
-  { simp only [h', exists_prop, insert_eq_of_mem],
-    exact ⟨t, subset.trans ss (subset_insert _ _), st, ct⟩ },
-  { refine ⟨insert a t, _⟩,
-    have ha := mt (@ss _) as,
-    rw [filter_map_insert_some f h],
-    refine ⟨insert_subset_insert _ ss, by rw st, _⟩,
-    rw [← st, card_insert_of_not_mem h', st, ct, card_insert_of_not_mem ha], }
-end
-
-def finset_embed {X : finset α} (S : finset {x // x ∈ X}) : finset α :=
-S.map $ function.embedding.subtype _
-
-lemma finset_embed_inj {X : finset α} : function.injective
-  (λ (S : finset {x // x ∈ X}), finset_embed S):=
-begin
-  unfold function.injective,
-  intros S T h,
-  simp only [ext, subtype.forall] at h ⊢,
-  intros a ha,
-  simp only [finset_embed, function.embedding.subtype, exists_prop,
-    exists_and_distrib_right, exists_eq_right, function.embedding.coe_fn_mk, mem_map,
-    subtype.exists] at h,
-  exact iff.intro (λ H, exists.elim ((h a).mp (exists.intro ha H)) (λ ha_, id))
-    (λ H, exists.elim ((h a).mpr (exists.intro ha H)) (λ ha_, id)),
-end
-
-instance finset_embed_coe (X : finset α) : has_coe (finset {x : α // x ∈ X}) (finset α) :=
-⟨finset_embed⟩
-
-def finset_finset_embed {X : finset α} (S : finset (finset {x // x ∈ X})) : finset (finset α) :=
-S.map $ ⟨finset_embed, finset_embed_inj⟩
-
-instance finset_finset_embed_coe (X : finset α) : has_coe (finset (finset {x : α // x ∈ X}))
-  (finset (finset α)) :=
-⟨finset_finset_embed⟩
-
--- need some basic theorems about finset_finset_embed_coe
-
-lemma finset_embed_coe_def {X : finset α} (S : finset {x // x ∈ X}) : ↑S = finset_embed S :=
-rfl
-
-lemma finset_finset_embed_coe_def {X : finset α} (S : finset (finset {x // x ∈ X})) : ↑S = finset_finset_embed S :=
-rfl
-
-/-lemma finset_embed_mem_univ {X : finset α} (x : finset {a // a ∈ X}) : (↑x : α) ∈ X :=
-begin
-end-/
-
-lemma finset_embed_subset_univ {X : finset α} (S : finset {a // a ∈ X}) : ↑S ⊆ X :=
-by { simp only [subset_iff, finset_embed_coe_def, finset_embed, function.embedding.subtype,
-    exists_prop, exists_and_distrib_right, exists_eq_right, function.embedding.coe_fn_mk,
-    mem_map, subtype.exists, exists_imp_distrib],
-  exact λ _ ha _, ha, }
-
-lemma finset_embed_mem {X : finset α} {S : finset {a : α // a ∈ X}} {x : {a : α // a ∈ X}} :
-  x ∈ S ↔ x.val ∈ (↑S : finset α) :=
-by { simp only [finset_embed_coe_def, finset_embed, function.embedding.subtype,
-    exists_prop, exists_and_distrib_right, subtype.eta, exists_eq_right,
-    function.embedding.coe_fn_mk, mem_map, subtype.exists],
-  exact iff.intro (λ h, ⟨x.2, mem_def.mp h⟩) (λ h, h.2), }
-
-/-lemma finset_embed_finset_mem {X : finset α} {S : finset (finset {a : α // a ∈ X})}
-  {x : finset {a : α // a ∈ X}} : x ∈ S ↔ ↑x ∈ (↑S) :=
-sorry-/
-/-
-lemma aux : insert e ↑x = ↑(insert e x) := sorry-/
-
-lemma finset_embed_subset {X : finset α} {x y : finset {a // a ∈ X}} :
-  x ⊆ y ↔ ↑x ⊆ (↑y : finset α) :=
-by { simp only [subset_iff, finset_embed_coe_def, finset_embed, function.embedding.subtype,
-    exists_prop, exists_and_distrib_right, exists_eq_right, function.embedding.coe_fn_mk,
-    mem_map, subtype.forall, subtype.exists, exists_imp_distrib],
-  exact iff.intro (λ h a ha H, exists.intro ha (h a ha H))
-    (λ h a ha H, exists.elim (h ha H) (λ ha_ hay, hay)), }
-
-lemma finset_embed_card [decidable_eq α] {X : finset α} (x : finset {a // a ∈ X}) : card x = card (↑x : finset α) :=
-by { rw [finset_embed_coe_def, finset_embed],
-  exact (map_eq_image (function.embedding.subtype _) x).symm ▸
-    (card_image_of_injective x (function.embedding.subtype _).2).symm, }
-
-section prestrict
-variables [decidable_eq α] [fintype α]
-
-/-- def by Mario Carneiro https://leanprover.zulipchat.com/#narrow/stream/113489-new-members/subject/finset.20of.20subtype.20from.20filter/near/134578668 -/
-def prestrict (X : finset α) (I : finset α) : option (finset {x : α // x ∈ X}) :=
-if h : _ then some
-  ⟨I.1.pmap (λ x h', ⟨x, h'⟩) h,
-    multiset.nodup_pmap (λ _ _ _ _, subtype.mk_eq_mk.1) I.2⟩ else none
-
-lemma prestrict_eq_none {X : finset α} (I : finset α) : prestrict X I = none ↔ ¬ I ⊆ X :=
-begin
-  split,
-  { intros h hIX,
-    by_cases H : ∀ a, a ∈ I.val → a ∈ X,
-    { change dite _ _ _ = none at h,
-      rw dif_pos H at h,
-      cases h, },
-    { rcases not_forall.1 H with ⟨x, hx⟩,
-      rw [not_imp, ←mem_def] at hx,
-      exact hx.2 (hIX hx.1), }, },
-  { intro hIX,
-    exact dif_neg hIX, },
-end
-
-lemma prestrict_eq_some_aux {X : finset α} {I : finset α} (h : ∀ a, a ∈ I.val → a ∈ X) :
-  let I' : finset {x // x ∈ X} :=
-    {val := multiset.pmap (λ x h', ⟨x, h'⟩) (I.val) h,
-    nodup := prestrict._proof_1 X I h} in
-  ↑I' = I :=
-begin
-  intro I',
-  rw [←val_inj, finset_embed_coe_def, finset_embed, map_val, multiset.map_pmap, le_antisymm_iff],
-  split,
-  { have hnodup := multiset.nodup_pmap _ I.2,
-    rw [multiset.le_iff_subset hnodup, multiset.subset_iff],
-    { intros x hx,
-      rw multiset.mem_pmap at hx,
-      rcases hx with ⟨a, haI, H⟩,
-      convert haI,
-      subst H,
-      refl, },
-    intros a ha b hb H,
-    have hinj : (⟨a, ha⟩ : {x // x ∈ X}) = ⟨b, hb⟩ := (function.embedding.subtype _).2 H,
-    exact subtype.mk_eq_mk.1 hinj, },
-  { rw [multiset.le_iff_subset I.2, multiset.subset_iff],
-    intros x hx,
-    rw multiset.mem_pmap,
-    use [x, hx],
-    refl, },
-end
-
-lemma prestrict_eq_some_of_subset {X : finset α} {I : finset α} (h : I ⊆ X)
-  : ∃ I', prestrict X I = some I' ∧ ↑I' = I :=
-begin
-  let I' := _,
-  have : prestrict X I = some I' := dif_pos h,
-  use [I', this],
-  exact prestrict_eq_some_aux h,
-end
-
-lemma subset_of_prestrict_eq_some {X : finset α} {I : finset α} {I' : finset {x : α // x ∈ X}}
-  (h : prestrict X I = some I') : I ⊆ X ∧ ↑I' = I :=
-begin
-  by_cases H : ∀ a, a ∈ I.val → a ∈ X,
-  { split,
-    { exact H, },
-    { change dite _ _ _ = _ at h,
-      rw [dif_pos H, option.some_inj] at h,
-      subst h,
-      exact prestrict_eq_some_aux H, }, },
-  { exfalso,
-    change dite _ _ _ = _ at h,
-    rw dif_neg H at h,
-    cases h, },
-end
-
-def prestrict_subset {X Y : finset α} (h : X ⊆ Y) : finset {x // x ∈ Y} :=
-sorry
-
-end prestrict
-
-variable [decidable_eq α]
-
-lemma inter_of_subset {A B : finset α} (h : A ⊆ B) : A ∩ B = A :=
-lattice.inf_of_le_left h
-
-lemma subset_iff_sdiff_eq_empty {x y : finset α} : x ⊆ y ↔ x \ y = ∅ :=
-by simp only [sdiff_eq_filter, eq_empty_iff_forall_not_mem, subset_iff, not_and,
-  not_not, finset.mem_filter]
-
-lemma empty_sdiff (E : finset α) : E \ ∅ = E :=
-by simp only [ext, finset.not_mem_empty, and_true, iff_self, finset.mem_sdiff,
-  not_false_iff, forall_true_iff]
-
-lemma sdiff_subset (A B : finset α): A \ B ⊆ A :=
-(empty_sdiff A).subst $ sdiff_subset_sdiff (subset.refl A) $ empty_subset B
-
-lemma sdiff_eq_sdiff_inter (A B : finset α) : A \ B = A \ (A ∩ B) :=
-by { simp only [ext, not_and, mem_sdiff, mem_inter],
-  exact λ a, iff.intro (λ h, ⟨h.1, λ x, h.2⟩) (λ h, ⟨h.1, h.2 h.1⟩), }
-
-lemma card_eq_inter_sdiff (A B : finset α) : card A = card (A ∩ B) + card (A \ B) :=
-begin
-  have hA : A \ B ∪ A ∩ B = A := by { simp only [ext, mem_union, union_comm, mem_sdiff, mem_inter],
-    exact λ a, iff.intro (λ ha, or.elim ha (λ H, H.1) (λ H, H.1))
-      (by { intro ha, by_cases h : a ∈ B, { exact or.inl ⟨ha, h⟩ }, { exact or.inr ⟨ha, h⟩ } }) },
-  have : disjoint (A \ B) (A ∩ B) := by simp only [disjoint, empty_subset, inf_eq_inter,
-    inter_empty, sdiff_inter_self, inter_left_comm, le_iff_subset],
-  replace this := card_disjoint_union this, rwa [hA, add_comm] at this,
-end
-
-lemma card_sdiff_eq (A B : finset α) : card (A \ B) = card A - card (A ∩ B) :=
-(nat.sub_eq_of_eq_add $ card_eq_inter_sdiff A B).symm
-
-lemma card_union_inter (A B : finset α) : card A + card B = card (A ∪ B) + card (A ∩ B) :=
-begin
-  have hBA : card B = card (B \ A) + card (A ∩ B) := inter_comm B A ▸
-    (add_comm (card (B ∩ A)) (card (B \ A))) ▸ (card_eq_inter_sdiff B A),
-  have Hdis : disjoint A (B \ A) := by simp only [disjoint, empty_subset, inf_eq_inter,
-    inter_sdiff_self, le_iff_subset],
-  have H : card A + card (B \ A) = card (A ∪ B) :=
-    (congr_arg card $ union_sdiff_self_eq_union.symm).substr (card_disjoint_union Hdis).symm,
-  calc
-  card A + card B = card A + card (B \ A) + card (A ∩ B) : by rw [add_assoc, hBA]
-  ... = card (A ∪ B) + card (A ∩ B) : by rw H,
-end
-
-/- proof by Kenny Lau https://leanprover.zulipchat.com/#narrow/stream/113489-new-members/subject/choosing.20from.20difference.20of.20finsets/near/133624012 -/
-lemma exists_sdiff_of_card_lt {x y : finset α} (hcard : card x < card y) : ∃ e : α, e ∈ y \ x :=
-suffices ∃ e ∈ y, e ∉ x, by simpa only [exists_prop, finset.mem_sdiff],
-by_contradiction $ λ H, not_le_of_lt hcard $ card_le_of_subset $ by simpa only [not_exists,
-  exists_prop, not_and, not_not] using H
-
-/- proof by chris hughes
-https://leanprover.zulipchat.com/#narrow/stream/113489-new-members/subject/maximal.20finset.20in.20finset.20of.20finsets/near/133905271 -/
-lemma max_fun_of_ne_empty {F : finset β} (func : β → ℕ) (h : F ≠ ∅) :
-  ∃ x ∈ F, ∀ g ∈ F, func g ≤ func x :=
-let ⟨n, hn⟩ := (max_of_ne_empty (mt image_eq_empty.1 h) : ∃ a, a ∈ finset.max (F.image func)) in
-let ⟨x, hx₁, hx₂⟩ := mem_image.1 (mem_of_max hn) in
-  ⟨x, hx₁, hx₂.symm ▸ λ g hg, le_max_of_mem (mem_image.2 ⟨g, hg, rfl⟩) hn⟩
-
-lemma min_fun_of_ne_empty {F : finset β} (func : β → ℕ) (h : F ≠ ∅) :
-  ∃ x ∈ F, ∀ g ∈ F, func x ≤ func g :=
-let ⟨n, hn⟩ := (min_of_ne_empty $ mt image_eq_empty.1 h : ∃ a, a ∈ finset.min (F.image func)) in
-let ⟨x, hx₁, hx₂⟩ := mem_image.1 (mem_of_min hn) in
-  ⟨x, hx₁, hx₂.symm ▸ λ g hg, min_le_of_mem (mem_image.2 ⟨g, hg, rfl⟩) hn⟩
-
-section inst
-
-variables {F : finset α} {Q : finset α → Prop} [decidable_pred Q] {P : α → Prop} [decidable_pred P]
-
-instance decidable_not_forall (c₁ : finset (finset α)) :
-  decidable (∃ x : finset α, ¬(x ∈ c₁ → ¬Q x)) :=
-decidable_of_iff (∃ x ∈ c₁, Q x) $ by simp only [exists_prop, not_forall_not]
-
-instance decidable_exists_and_mem : decidable (∃ e, e ∈ F ∧ P e) :=
-decidable_of_iff (∃ e ∈ F, P e) $ by simp only [exists_prop]
-
-end inst
-
-end finset
+-/
 
 open finset
 
--- § 1.1
+/-! § 1.1 Independent sets and circuits.
+-/
 
 namespace matroid
 
 variables (E : Type*) [decidable_eq E] [fintype E]
 
-/-- `indep E` is the type of matroids (in the independent set representation)
-with ground set `E` (encoded in Lean as a fintype). -/
+/-- `of_indep E` is the type of matroids in the independent set representation
+with ground set `E` (encoded in Lean as a `fintype`).
+
+It has the following fields:
+- `indep : finset (finset E)` : the set of independent subsets of E
+- `empty_mem_indep` : axiom (I1), the empty set is independent.
+- `indep_of_subset_indep` : axiom (I2), subsets of independent sets are independent.
+- `indep_exch` : axiom (I3), the exchange axiom. Given two independent sets `x`, `y` with `x.card < y.card`, there exists `e ∈ y \ x` such that `insert e x` is independent.
+-/
 structure of_indep :=
 (indep : finset (finset E))
 -- (I1)
 (empty_mem_indep : ∅ ∈ indep)
 -- (I2)
-(indep_of_subset_indep {x y} (hx : x ∈ indep) (hyx : y ⊆ x) : y ∈ indep)
+(indep_of_subset_indep {x y : finset E} (hx : x ∈ indep) (hyx : y ⊆ x) : y ∈ indep)
 -- (I3)
 (indep_exch {x y : finset E} (hx : x ∈ indep) (hy : y ∈ indep) (hcard : card x < card y)
-    : ∃ e, e ∈ y \ x ∧ insert e x ∈ indep)
-
+  : ∃ e, e ∈ y \ x ∧ insert e x ∈ indep)
 
 namespace of_indep
 
+/-- independent set matroids are printed by printing their independent sets -/
 instance repr [has_repr E] : has_repr (of_indep E) :=
 ⟨λ m, has_repr.repr m.indep⟩
 
 variable {E}
 
-theorem eq_of_indep_eq : ∀ {M₁ M₂ : of_indep E}, M₁.1 = M₂.1 → M₁ = M₂
+/-- two independent set matroids are equal if their independent sets agree -/
+lemma eq_of_indep_eq : ∀ {M₁ M₂ : of_indep E}, M₁.1 = M₂.1 → M₁ = M₂
   | ⟨I₁, p₁, q₁, r₁⟩ ⟨I₂, p₂, q₂, r₂⟩ h :=
 by simpa only []
 
-/-- A circuit of a matroid is a minimal dependent subset of the ground set -/
+/-- A circuit of an independent set matroid is a minimal dependent subset of
+the ground set, i.e. all of its proper subsets are independent. -/
 def is_circuit (x : finset E) (m : of_indep E) : Prop :=
 x ∉ m.indep ∧ ∀ y, y ⊂ x → y ∈ m.indep
 
-/-- proof by Mario Carneiro https://leanprover.zulipchat.com/#narrow/stream/113489-new-members/subject/finsets.2C.20decidable_mem.2C.20and.20filter/near/133708937 -/
+/-- The property of being a circuit is decidable.
+
+proof by Mario Carneiro https://leanprover.zulipchat.com/#narrow/stream/113489-new-members/subject/finsets.2C.20decidable_mem.2C.20and.20filter/near/133708937 -/
 instance decidable_circuit (x : finset E) (m : of_indep E) : decidable (is_circuit x m) :=
-decidable_of_iff (x ∉ m.indep ∧ ∀ y ∈ (powerset x).erase x, y ∈ m.indep)
+decidable_of_iff (x ∉ m.indep ∧ ∀ y ∈ x.powerset.erase x, y ∈ m.indep)
 begin
   simp only [is_circuit, has_ssubset.ssubset, mem_powerset, and_imp, mem_erase],
   refine and_congr iff.rfl (forall_congr $ λ y, _),
@@ -384,33 +77,24 @@ begin
   { rintro rfl, refl }, { exact subset.antisymm h₂, },
 end
 
+/-- The property of containing a circuit as a subset is decidable -/
 instance decidable_circuit_subset (x : finset E) (m : of_indep E) :
   decidable (∃ (y : finset E) (H : y ⊆ x), is_circuit y m) :=
-decidable_of_iff (∃ (y : finset E) (H : y ∈ powerset x), is_circuit y m) $
+decidable_of_iff (∃ (y : finset E) (H : y ∈ x.powerset), is_circuit y m) $
   by simp only [exists_prop, mem_powerset]
 
-/- should I make this definition reducible? I don't know when to use attributes... -/
-def circuits_circuits (m : of_indep E) : finset (finset E) :=
-(powerset univ).filter (λ S, is_circuit S m)
+/-- the set of all circuits of the independent set matroid `m` -/
+def circuits (m : of_indep E) : finset (finset E) :=
+univ.powerset.filter (λ S, is_circuit S m)
 
-lemma C2 (m : of_indep E) (x y : finset E) (hx : x ∈ circuits_circuits m)
-  (hy : y ∈ circuits_circuits m) (hxy : x ⊆ y) : x = y :=
-begin
-  simp only [circuits_circuits, is_circuit, mem_filter] at hx hy hxy,
-  have hnxy : ¬x ⊂ y := λ h, hx.2.1 $ hy.2.2 x h,
-  rw ←lt_iff_ssubset at hnxy,
-  rw [←le_iff_subset, le_iff_eq_or_lt] at hxy,
-  cases hxy,
-  { exact hxy, },
-  { exact (hnxy hxy).elim, },
-end
-
+/-- A subset of the ground set is dependent if and only if it is contained
+in a circuit. -/
 theorem dep_iff_circuit_subset (x : finset E) (m : of_indep E) :
   x ∉ m.indep ↔ ∃ y ⊆ x, is_circuit y m :=
 begin
   split,
   { intro hxd,
-    rcases min_fun_of_ne_empty card (ne_empty_of_mem $
+    rcases min_fun_of_nonempty card (nonempty_of_mem $
       mem_filter.mpr ⟨mem_powerset.mpr $ subset.refl x, hxd⟩) with ⟨a, ha, hamin⟩,
     have hax : a ⊆ x := mem_powerset.mp (mem_filter.mp ha).1,
     use [a, hax], split,
@@ -419,74 +103,9 @@ begin
       refine not_le_of_lt (card_lt_card hy) _,
       refine hamin y (mem_filter.mpr ⟨_, h⟩),
       refine mem_powerset.mpr (subset.trans _ hax),
-      exact (le_of_lt $ lt_iff_ssubset.mpr hy), } },
+      exact (le_of_lt $ lt_iff_ssubset.mpr hy), }, },
   { rintros ⟨a, ⟨hax, hacirc⟩⟩ hxi,
     exact hacirc.1 (m.indep_of_subset_indep hxi hax), },
-end
-
-/-- Lemma 1.1.3 -/
-lemma C3 (m : of_indep E) (x y : finset E) (e : E) (hx : x ∈ m.circuits_circuits)
-  (hy : y ∈ m.circuits_circuits) (hxny : x ≠ y) (he : e ∈ x ∩ y) :
-  ∃ z, z ∈ m.circuits_circuits ∧ z ⊆ erase (x ∪ y) e :=
-begin
-  have hxmy : x \ y ≠ ∅ := mt subset_iff_sdiff_eq_empty.mpr (mt (m.C2 x y hx hy) hxny),
-  rcases exists_mem_of_ne_empty hxmy with ⟨a, ha⟩, clear hxny hxmy,
-  simp only [circuits_circuits, mem_powerset, mem_filter, mem_sdiff, mem_inter]
-    at ha hx hy he,
-  have hxai : erase x a ∈ m.indep := by { unfold is_circuit at hx,
-    exact hx.2.2 (erase x a) (erase_ssubset ha.1) },
-  let F := (powerset (x ∪ y)).filter (λ S, erase x a ⊆ S ∧ S ∈ m.indep),
-  have hxaF : erase x a ∈ F := mem_filter.2 ⟨mem_powerset.mpr $ subset.trans (erase_subset a x) $
-    subset_union_left x y, ⟨subset.refl _, hxai⟩⟩, clear hxai,
-  rcases (max_fun_of_ne_empty card $ ne_empty_of_mem hxaF) with ⟨I, ⟨hIF, hI⟩⟩, clear hxaF,
-  have hIFindep : I ∈ m.indep := (mem_filter.mp hIF).2.2,
-  have hIdep : _ → I ∉ m.indep := (dep_iff_circuit_subset I m).2,
-  have hIFxa : erase x a ⊆ I := (mem_filter.mp hIF).2.1,
-  have hIxuy : I ⊆ x ∪ y := mem_powerset.mp (mem_filter.mp hIF).1,
-  have haniI : a ∉ I :=
-    λ H, have hxI : x ⊆ I := (insert_erase ha.1) ▸ insert_subset.mpr ⟨H, hIFxa⟩,
-      have ∃ A ⊆ I, is_circuit A m := exists.intro x (exists.intro hxI hx.2),
-      hIdep this hIFindep,
-  have hEg : ∃ g ∈ y, g ∉ I :=
-    by { have hIdep2 := mt hIdep, simp only [not_exists, exists_prop, not_and, not_not]
-      at hIdep2,
-    have hyI0 := mt (hIdep2 hIFindep y), simp only [not_not] at hyI0,
-    have hYI : ¬y ⊆ I := hyI0 hy.2,
-    have this := exists_mem_of_ne_empty (mt subset_iff_sdiff_eq_empty.mpr hYI),
-    simp only [mem_sdiff] at this, simpa only [exists_prop], },
-  rcases hEg with ⟨g, ⟨hgy, hgnI⟩⟩, clear hIdep,
-  have hga : g ≠ a := λ H, ha.2 (H ▸ hgy),
-  have hIag : I ⊆ erase (erase (x ∪ y) a) g :=
-    subset_iff.mpr (λ xx hxx, mem_erase.mpr ⟨λ hgg, hgnI $ hgg ▸ hxx,
-      mem_erase.mpr ⟨λ hgga, haniI $ hgga ▸ hxx, mem_of_subset hIxuy hxx⟩⟩),
-  have haxuy : a ∈ x ∪ y := mem_union_left y ha.1,
-  have hcardxye : card (erase (x ∪ y) a) = nat.pred (card (x ∪ y)) :=
-    card_erase_of_mem haxuy,
-  have hpcard : nat.pred (card (x ∪ y)) > 0 := by { rw ←hcardxye,
-    exact card_pos.mpr (ne_empty_of_mem $ mem_erase.mpr ⟨hga, mem_union_right x hgy⟩), },
-  have hcard : card I < card (erase (x ∪ y) e) :=
-    calc card I ≤ card (erase (erase (x ∪ y) a) g) : card_le_of_subset hIag
-    ... = nat.pred (nat.pred (card (x ∪ y))) : by rw [card_erase_of_mem
-      (mem_erase.mpr ⟨hga, mem_union_right x hgy⟩), hcardxye]
-    ... < card (erase (x ∪ y) e) :
-      by { rw [card_erase_of_mem (mem_union_left y he.1),
-      ←nat.succ_pred_eq_of_pos hpcard], exact nat.lt_succ_self _, },
-  clear hga hIag haxuy hcardxye hpcard he,
-  by_contra h, simp only [circuits_circuits, mem_powerset, not_exists, and_imp,
-    mem_filter, not_and] at h,
-  have : (∀ x_1 : finset E, x_1 ⊆ erase (x ∪ y) e → ¬is_circuit x_1 m) :=
-    λ x1 hx1, (mt $ h x1 $ subset_univ x1) $ not_not.mpr hx1,
-  have hindep := mt (dep_iff_circuit_subset (erase (x ∪ y) e) m).mp,
-  simp only [not_exists, exists_prop, not_and, not_not] at hindep,
-  replace hindep : erase (x ∪ y) e ∈ m.indep := hindep this,
-  rcases (m.indep_exch hIFindep hindep hcard) with ⟨El, ⟨hElxy, hElindep⟩⟩,
-  have hElF : insert El I ∈ F := mem_filter.mpr ⟨mem_powerset.mpr
-    (insert_subset.mpr ⟨(mem_erase.mp (mem_sdiff.mp hElxy).1).2, hIxuy⟩),
-    ⟨subset.trans hIFxa (subset_insert El I), hElindep⟩⟩,
-  have hcardEl : card I < card (insert El I) :=
-    by { rw card_insert_of_not_mem (mem_sdiff.mp hElxy).2,
-    exact lt_add_one (card I), },
-  exact not_lt.mpr (hI (insert El I) hElF) hcardEl,
 end
 
 end of_indep
@@ -494,25 +113,35 @@ end of_indep
 open of_indep
 variable (E)
 
+/-- `of_circuits E` is the type of matroids in the circuit representation with ground set `E` (encoded in Lean as a fintype).
+
+It has the following fields:
+- `circuits : finset (finset E)` : the set of circuits of E
+- `empty_not_mem_circuits` : axiom (C1), the empty set is not a circuit.
+- `circuits_eq_of_subset` : axiom (C2), if `x` and `y` are circuits and `x ⊆ y` then `x = y`.
+- `circuit_elim` : axiom (C3), the (weak) circuit elimination axiom.
+  Given two unequal circuits `x`, `y` and an element `e ∈ x ∩ y`, there exists a circuit `z ⊆ (x ∪ y).erase e`.
+ -/
 structure of_circuits :=
 (circuits : finset (finset E))
 -- (C1)
 (empty_not_mem_circuits : ∅ ∉ circuits)
 -- (C2)
-(circuits_eq_of_subset {x y} (hx : x ∈ circuits) (hy : y ∈ circuits) (hxy : x ⊆ y) : x = y)
+(circuits_eq_of_subset {x y : finset E} (hx : x ∈ circuits) (hy : y ∈ circuits) (hxy : x ⊆ y) : x = y)
 -- (C3)
-(circuit_elim {x y e} (hx : x ∈ circuits) (hy : y ∈ circuits) (hxy : x ≠ y) (he : e ∈ x ∩ y) :
-  ∃ z, z ∈ circuits ∧ z ⊆ erase (x ∪ y) e)
---attribute [class] circuits
+(circuit_elim {x y : finset E} {e : E} (hx : x ∈ circuits) (hy : y ∈ circuits) (hxy : x ≠ y) (he : e ∈ x ∩ y) :
+  ∃ z, z ∈ circuits ∧ z ⊆ (x ∪ y).erase e)
 
 namespace of_circuits
 
+/-- circuit matroids are printed by printing their circuits -/
 instance repr [has_repr E] : has_repr (of_circuits E) :=
 ⟨λ c, has_repr.repr c.circuits⟩
 
 variable {E}
 
-theorem eq_of_circ_eq : ∀ {C₁ C₂ : of_circuits E}, C₁.1 = C₂.1 → C₁ = C₂
+/-- two circuit matroids are equal if they have the same sets of circuits -/
+lemma eq_of_circ_eq : ∀ {C₁ C₂ : of_circuits E}, C₁.1 = C₂.1 → C₁ = C₂
   | ⟨c₁, p₁, q₁, r₁⟩ ⟨c₂, p₂, q₂, r₂⟩ h :=
 by simpa only []
 
@@ -522,16 +151,120 @@ namespace of_indep
 
 variable {E}
 
-def circuits (m : of_indep E) : of_circuits E :=
-{ circuits := m.circuits_circuits,
+/-- "it is easy to see that..."
+If x and y are members of m.circuits,  and x ⊆ y, then x = y.
+-/
+private lemma C2 (m : of_indep E) (x y : finset E) (hx : x ∈ m.circuits)
+  (hy : y ∈ m.circuits) (hxy : x ⊆ y) : x = y :=
+begin
+  simp only [circuits, is_circuit, mem_filter] at hx hy hxy,
+  have hnxy : ¬x ⊂ y := λ h, hx.2.1 $ hy.2.2 x h,
+  rw [←le_iff_subset, le_iff_eq_or_lt] at hxy,
+  cases hxy,
+  { exact hxy, },
+  { exact (hnxy hxy).elim, },
+end
+
+/-- Lemma 1.1.3. If `x` and `y` are distinct members of `m.circuits` and `e ∈ x ∩ y`,
+then there is a member `z` of `m.circuits` such that `z ⊆ (x ∪ y).erase e` -/
+private lemma C3 (m : of_indep E) (x y : finset E) (e : E) (hx : x ∈ m.circuits)
+  (hy : y ∈ m.circuits) (hxny : x ≠ y) (he : e ∈ x ∩ y) :
+  ∃ z, z ∈ m.circuits ∧ z ⊆ (x ∪ y).erase e :=
+begin
+  -- by C2, `y - x` is nonempty,
+  have hxmy : (x \ y).nonempty := nonempty_of_ne_empty
+    (mt subset_iff_sdiff_eq_empty.mpr (mt (C2 m x y hx hy) hxny)), clear hxny,
+  -- so we can choose an element `a` from this set
+  rcases hxmy with ⟨a, ha⟩,
+  simp only [circuits, mem_powerset, mem_filter, mem_sdiff, mem_inter]
+    at ha hx hy he,
+  -- as `x` is a minimal dependent set, `x.erase a ∈ m.indep`
+  have hxai : x.erase a ∈ m.indep := by { unfold is_circuit at hx,
+    exact hx.2.2 (x.erase a) (erase_ssubset ha.1) },
+  -- consider the set F of all subsets of `x ∪ y` which
+  -- contain `x.erase a` and are independent
+  let F := (x ∪ y).powerset.filter (λ S, x.erase a ⊆ S ∧ S ∈ m.indep),
+  -- F contains `x.erase a`
+  have hxaF : x.erase a ∈ F := mem_filter.2 ⟨mem_powerset.mpr $ subset.trans (x.erase_subset a) $
+    subset_union_left x y, ⟨subset.refl _, hxai⟩⟩, clear hxai,
+  -- hence F is nonempty and we can choose a maximal subset `I` from `F`
+  rcases (max_fun_of_nonempty card $ nonempty_of_mem hxaF) with ⟨I, ⟨hIF, hI⟩⟩, clear hxaF,
+  have hIxuy : I ⊆ x ∪ y := mem_powerset.mp (mem_filter.mp hIF).1,
+  have hIFindep : I ∈ m.indep := (mem_filter.mp hIF).2.2,
+  have hIFxa : x.erase a ⊆ I := (mem_filter.mp hIF).2.1,
+  -- if we can find a subset of `I` that is a circuit, we have a contradiction
+  have hIdep : _ → I ∉ m.indep := (dep_iff_circuit_subset I m).2,
+  have haniI : a ∉ I := by { intro H,
+    have hxI : x ⊆ I := (insert_erase ha.1) ▸ insert_subset.mpr ⟨H, hIFxa⟩,
+    refine hIdep _ hIFindep,
+    use [x, hxI], exact hx.2, }, clear hx,
+  -- since `y` is a circuit, some element `g` of `y` is not in `I`
+  have hEg : ∃ g ∈ y, g ∉ I :=
+    by { have hIdep2 := mt hIdep, simp only [not_exists, exists_prop, not_and, not_not]
+      at hIdep2,
+    have hyI0 := mt (hIdep2 hIFindep y), simp only [not_not] at hyI0,
+    have hYI : ¬y ⊆ I := hyI0 hy.2, clear hyI0,
+    have : ∃ x, x ∈ y \ I := (nonempty_of_ne_empty (mt subset_iff_sdiff_eq_empty.mpr hYI)).bex,
+    simp only [mem_sdiff] at this, simpa only [exists_prop], }, clear hy hIdep,
+  rcases hEg with ⟨g, ⟨hgy, hgnI⟩⟩,
+  -- as `a ∈ x.erase y`, `a` and `g` are distinct
+  have hga : g ≠ a := λ H, ha.2 (H ▸ hgy),
+  have hIag : I ⊆ ((x ∪ y).erase a).erase g :=
+    subset_iff.mpr (λ xx hxx, mem_erase.mpr ⟨λ hgg, hgnI $ hgg ▸ hxx,
+      mem_erase.mpr ⟨λ hgga, haniI $ hgga ▸ hxx, mem_of_subset hIxuy hxx⟩⟩),
+  have haxuy : a ∈ x ∪ y := mem_union_left y ha.1, clear ha,
+  have hcardxye : ((x ∪ y).erase a).card = (x ∪ y).card.pred :=
+    card_erase_of_mem haxuy, clear haxuy,
+  have hpcard : (x ∪ y).card.pred > 0 := by { rw ←hcardxye,
+    exact card_pos.mpr (nonempty_of_mem $ mem_erase.mpr ⟨hga, mem_union_right x hgy⟩), },
+  -- we show the inequality `I.card < ((x ∪ y).erase e).card`
+  have hcard : I.card < ((x ∪ y).erase e).card :=
+    calc I.card ≤ (((x ∪ y).erase a).erase g).card : card_le_of_subset hIag
+    ... = (x ∪ y).card.pred.pred : by rw [card_erase_of_mem
+      (mem_erase.mpr ⟨hga, mem_union_right x hgy⟩), hcardxye]
+    ... < ((x ∪ y).erase e).card :
+      by { rw [card_erase_of_mem (mem_union_left y he.1),
+      ←nat.succ_pred_eq_of_pos hpcard], exact nat.lt_succ_self _, },
+  clear hga hIag hcardxye hpcard he hgy hgnI g,
+  -- assume that `(x ∪ y).erase e` does not contain a circuit
+  by_contra h, simp only [circuits, mem_powerset, not_exists, and_imp,
+    mem_filter, not_and] at h,
+  have : (∀ x' : finset E, x' ⊆ (x ∪ y).erase e → ¬is_circuit x' m) :=
+    λ x1 hx1, (mt $ h x1 $ subset_univ x1) $ not_not.mpr hx1,
+  -- then `(x ∪ y).erase e` is independent
+  have hindep := mt (dep_iff_circuit_subset ((x ∪ y).erase e) m).mp,
+  simp only [not_exists, exists_prop, not_and, not_not] at hindep,
+  replace hindep : (x ∪ y).erase e ∈ m.indep := hindep this, clear this,
+  -- now apply I3, taking `x` and `y` to be `I` and `(x ∪ y).erase e`, respectively
+  rcases (m.indep_exch hIFindep hindep hcard) with ⟨El, ⟨hElxy, hElindep⟩⟩,
+  clear hcard hIFindep hindep,
+  -- the resulting independent set `insert El I` is in `F`
+  have hElF : insert El I ∈ F := mem_filter.mpr ⟨mem_powerset.mpr
+    (insert_subset.mpr ⟨(mem_erase.mp (mem_sdiff.mp hElxy).1).2, hIxuy⟩),
+    ⟨subset.trans hIFxa (subset_insert El I), hElindep⟩⟩,
+  -- and is larger than `I`
+  have hcardEl : I.card < (insert El I).card :=
+    by { rw card_insert_of_not_mem (mem_sdiff.mp hElxy).2,
+    exact lt_add_one I.card, },
+  -- which contradicts the maximality of `I`
+  exact not_lt.mpr (hI (insert El I) hElF) hcardEl,
+end
+
+/-- `m.to_circuits` constructs the circuit matroid from the independent sets
+matroid `m` -/
+def to_circuits (m : of_indep E) : of_circuits E :=
+{ circuits := m.circuits,
   empty_not_mem_circuits :=
     begin
-      simp only [circuits_circuits, is_circuit, mem_filter, not_and],
+      simp only [circuits, is_circuit, mem_filter, not_and],
       intros h h1, exfalso,
       exact h1 m.empty_mem_indep,
     end,
-  circuits_eq_of_subset := m.C2,
-  circuit_elim := m.C3 }
+  circuits_eq_of_subset := C2 m,
+  circuit_elim := C3 m }
+
+@[simp] lemma to_circuits_circuits_eq_circuits (m : of_indep E) :
+  m.to_circuits.circuits = m.circuits := rfl
 
 end of_indep
 
@@ -539,51 +272,68 @@ namespace of_circuits
 open of_indep
 variable {E}
 
-/- make reducible? -/
-def indep_indep (C : of_circuits E) : finset (finset E) :=
-(powerset univ).filter (λ S, ∀ c ∈ C.circuits, ¬c ⊆ S)
+/-- all independent sets of the matroid `C` in the circuit representation.
+These are the subsets of the ground set `E` which contain no circuit.
+-/
+def indep (C : of_circuits E) : finset (finset E) :=
+univ.powerset.filter (λ S, ∀ c ∈ C.circuits, ¬c ⊆ S)
 
-/-- first part of Theorem 1.1.4 -/
-lemma I2 (C : of_circuits E) (x y : finset E) : x ∈ C.indep_indep → y ⊆ x →
-  y ∈ C.indep_indep :=
+/-- first part of Theorem 1.1.4: Let `E` be a set and `C` be a collection of subsets
+of `E` satisfying C1-C3. Let `I` be the collection of subsets of `E` that contain
+no member of `C`. Then `(E,I)` satisfies C2 -/
+private lemma I2 (C : of_circuits E) (x y : finset E) : x ∈ C.indep → y ⊆ x →
+  y ∈ C.indep :=
 begin
-  simp only [indep_indep, mem_powerset, and_imp, mem_filter],
-  exact λ hxE hx hxy, ⟨subset.trans hxy hxE, λ c hc H, hx c hc $ subset.trans H hxy⟩,
+  simp only [indep, mem_powerset, and_imp, mem_filter],
+  intros _ hx hxy, split, { exact subset_univ y, },
+  { intros c hc H, exact hx c hc (subset.trans H hxy), },
 end
 
-/-- second part of Theorem 1.1.4 -/
-lemma I3 (C : of_circuits E) (x y : finset E) (hx : x ∈ C.indep_indep)
-  (hy : y ∈ C.indep_indep) (hcardxy : card x < card y)
-  : ∃ e, e ∈ y \ x ∧ insert e x ∈ C.indep_indep :=
+/-- second part of Theorem 1.1.4; Let `E` be a set and `C` be a collection of subsets
+of `E` satisfying C1-C3. Let `I` be the collection of subsets of `E` that contain
+no member of `C`. Then `(E,I)` satisfies C3 -/
+private lemma I3 (C : of_circuits E) (x y : finset E)
+  -- Let `x` and `y` be members of `I` and `x.card < y.card`
+  (hx : x ∈ C.indep) (hy : y ∈ C.indep) (hcardxy : x.card < y.card)
+  : ∃ e, e ∈ y \ x ∧ insert e x ∈ C.indep :=
 begin
-  unfold indep_indep at ⊢,
-  simp only [indep_indep, mem_powerset, mem_filter] at hx hy,
+  unfold indep at ⊢,
+  simp only [indep, mem_powerset, mem_filter] at hx hy,
+  -- assume I3 fails for the pair (x,y)
   by_contra h,
   simp only [mem_powerset, not_exists, and_imp, mem_filter, not_and, mem_sdiff] at h,
-  let F := (powerset $ x ∪ y).filter (λ S, (∀ c ∈ C.circuits, ¬c ⊆ S) ∧ card x < card S),
+  -- consider the set `F` of all subsets of `x ∪ y` which are members of `I` with more elements than `x`
+  let F := (x ∪ y).powerset.filter (λ S, (∀ c ∈ C.circuits, ¬c ⊆ S) ∧ x.card < S.card),
+  -- `F` contains `y` and is nonempty
   have hyF : y ∈ F := mem_filter.mpr ⟨mem_powerset.mpr $ subset_union_right x y,
     ⟨hy.2, hcardxy⟩⟩,
-  rcases (min_fun_of_ne_empty (λ f, card (x \ f)) $ ne_empty_of_mem hyF) with ⟨z, ⟨hz, hminz⟩⟩,
+  -- choose a subset `z` contained in `F` such that `(x \ z).card` is minimal
+  rcases (min_fun_of_nonempty (λ f, (x \ f).card) $ nonempty_of_mem hyF) with ⟨z, ⟨hz, hminz⟩⟩,
   clear hcardxy hyF,
   have hzxuy : z ⊆ x ∪ y := mem_powerset.mp (mem_filter.mp hz).1,
   replace hz := (mem_filter.mp hz).2,
-  rcases (exists_sdiff_of_card_lt hz.2) with ⟨a, ha⟩,
+  -- let `a` be an element of `z \ x`
+  rcases (nonempty_sdiff_of_card_lt hz.2) with ⟨a, ha⟩,
   rw mem_sdiff at ha,
-  have hxsdiffz : x \ z ≠ ∅ :=
-    by { intro H,
+  -- "since I3 fails, `x \ z` is nonempty"...
+  have hxsdiffz : (x \ z).nonempty :=
+    by { apply nonempty_of_ne_empty, intro H,
     have Hxsubz : x ⊆ z := subset_iff_sdiff_eq_empty.mpr H,
-    have hay : a ∈ y := or.elim (mem_union.mp $ mem_of_subset hzxuy ha.1)
-      (λ Hax, false.elim $ ha.2 Hax) id,
-    have haindep : insert a x ∈ C.indep_indep := C.I2 z (insert a x)
-      (by { simp only [indep_indep, mem_powerset, mem_filter],
-      exact ⟨subset.trans hzxuy $ union_subset hx.1 hy.1, hz.1⟩, })
+    have hay : a ∈ y := (mem_union.mp $ mem_of_subset hzxuy ha.1).elim
+      (λ Hax, (ha.2 Hax).elim) id,
+    have haindep : insert a x ∈ C.indep := I2 C z (insert a x)
+      (by { simp only [indep, mem_powerset, mem_filter],
+      exact ⟨subset_univ z, hz.1⟩, })
       (insert_subset.mpr ⟨ha.1, Hxsubz⟩),
-    simp only [indep_indep, mem_powerset, mem_filter] at haindep,
+    simp only [indep, mem_powerset, mem_filter] at haindep,
+    -- [`h` is the negation of I3]
     exact h a hay ha.2 haindep.1 haindep.2, },
-  rcases (exists_mem_of_ne_empty hxsdiffz) with ⟨e, he⟩,
-  clear h ha hxsdiffz,
+  -- choose an element `e` from `x \ z`
+  rcases hxsdiffz with ⟨e, he⟩, clear h ha,
   rw mem_sdiff at he,
-  let T : E → finset E := λ f, erase (insert e z) f,
+  -- for each `f`, let T_f be `(insert e z).erase f`
+  let T : E → finset E := λ f, (insert e z).erase f,
+  -- for each `f` in `z \ x`, `T f` is in `x ∪ y` and
   have hTf1 : ∀ f, f ∈ z \ x → T f ⊆ x ∪ y :=
     by { intros f hf, rw [mem_sdiff] at hf,
     rw [subset_iff],
@@ -591,8 +341,9 @@ begin
     simp only [mem_union],
     rcases hgg.2 with rfl | hggz,
     { exact or.inl he.1, },
-    exact (mem_union.mp $ mem_of_subset hzxuy hggz) },
-  have hTf2 : ∀ f, f ∈ z \ x → card (x \ T f) < card (x \ z) :=
+    exact (mem_union.mp $ mem_of_subset hzxuy hggz), },
+  -- for each `f` in `z \ x`, we have `(x \ T f).card < (x \ z).card`
+  have hTf2 : ∀ f, f ∈ z \ x → (x \ T f).card < (x \ z).card :=
     by { intros f hf, rw mem_sdiff at hf,
     suffices H : x \ T f ⊂ x \ z, exact card_lt_card H,
     by { simp only [ssubset_iff, exists_prop, mem_insert, not_forall_not, not_and,
@@ -600,54 +351,64 @@ begin
       use e, split,
       { intro _, split,
         { intro hef, exact hf.2 (hef ▸ he.1), },
-        { exact or.inl rfl, } },
+        { exact or.inl rfl, }, },
       { rw [subset_iff],
         intros gg hgg,
         simp only [mem_insert, not_and, mem_sdiff, mem_erase, ne.def] at hgg,
         have ggnef : gg ≠ f := by { intro ggef,
           rcases hgg with gge | H,
           { exact ((gge.symm ▸ he.2) $ ggef.substr hf.1), },
-          { exact (ggef.substr hf.2) H.1, } },
+          { exact (ggef.substr hf.2) H.1, }, },
         have he0 : e ∈ x \ z := mem_sdiff.mpr he,
         rcases hgg with gge | H,
         { exact gge.symm ▸ he0, },
-        { exact mem_sdiff.mpr ⟨H.1, λ ggz, (H.2 ggnef) $ or.inr ggz⟩, } } } },
-  have hTfindep : ∀ f, f ∈ z \ x → T f ∉ C.indep_indep :=
+        { exact mem_sdiff.mpr ⟨H.1, λ ggz, (H.2 ggnef) $ or.inr ggz⟩, }, }, }, },
+  -- Therefore `T f` is not in `C.indep`
+  have hTfindep : ∀ f, f ∈ z \ x → T f ∉ C.indep :=
     by { intros f hf,
-    simp only [indep_indep, mem_powerset, mem_filter, not_and],
+    simp only [indep, mem_powerset, mem_filter, not_and],
     intros hTfE H,
     have HTf1 : T f ⊆ x ∪ y := hTf1 f hf,
-    have HTf2 : card (x \ T f) < card (x \ z) := hTf2 f hf,
+    have HTf2 : (x \ T f).card < (x \ z).card := hTf2 f hf,
     rw mem_sdiff at hf,
-    have HTfcard : card z = card (T f) :=
+    have HTfcard : z.card = (T f).card :=
       by { simp only [card_erase_of_mem (mem_insert.mpr $ or.inr hf.1),
       card_insert_of_not_mem he.2, mem_insert, card_insert_of_not_mem, nat.pred_succ], },
-    replace HTfcard : card x < card (T f) := HTfcard ▸ hz.2,
+    replace HTfcard : x.card < (T f).card := HTfcard ▸ hz.2,
     have : T f ∈ F := mem_filter.mpr ⟨mem_powerset.mpr HTf1, ⟨H, HTfcard⟩⟩,
     exact not_lt.mpr (hminz (T f) this) HTf2, },
+  -- so `T f` contains a member C_f of `C.circuits`
   have hTfC : ∀ f, f ∈ z \ x → ∃ c ∈ C.circuits, c ⊆ T f :=
     by { intros f hf,
-    have : T f ∉ C.indep_indep := hTfindep f hf,
-      simp only [indep_indep, mem_powerset, mem_filter, not_and] at this,
+    have : T f ∉ C.indep := hTfindep f hf,
+      simp only [indep, mem_powerset, mem_filter, not_and] at this,
     have hfc := this (subset.trans (hTf1 f hf) $ union_subset hx.1 hy.1),
     by_contra H, simp only [not_exists, exists_prop, not_and] at H, contradiction, },
-  rcases (exists_sdiff_of_card_lt hz.2) with ⟨g, hg⟩,
+  -- Let `g` be an element of `z \ x`
+  rcases (nonempty_sdiff_of_card_lt hz.2) with ⟨g, hg⟩,
+  -- and let C_g be the circuit contained in T g
   rcases (hTfC g hg) with ⟨Cg, ⟨HCg1, HCg2⟩⟩,
   clear hTf1 hTf2 hTfindep hg hy hminz hzxuy,
-  have hCgsub : Cg ⊆ insert e z := subset.trans HCg2 (erase_subset g $ insert e z),
+  have hCgsub : Cg ⊆ insert e z := subset.trans HCg2 ((insert e z).erase_subset g),
   rw [subset_iff] at HCg2,
-  have HCgzx : Cg ∩ (z \ x) ≠ ∅ := by { intro H,
+  have HCgzx : (Cg ∩ (z \ x)).nonempty := by {
+    apply nonempty_of_ne_empty,
+    -- if `Cg ∩ (z \ x) = ∅`,
+    intro H,
+    -- then `Cg ⊆ x` leads to a contradiction
     suffices : Cg ⊆ x, from hx.2 Cg HCg1 this,
-    suffices H1 : Cg ⊆ erase (insert e (x ∩ z)) g, from
-    suffices H2 : erase (insert e (x ∩ z)) g ⊆ x, from
+    -- we show this by showing `Cg ⊆ (insert e (x ∩ z)).erase g`
+    suffices H1 : Cg ⊆ (insert e (x ∩ z)).erase g, from
+    -- and `(insert e (x ∩ z)).erase g ⊆ x`
+    suffices H2 : (insert e (x ∩ z)).erase g ⊆ x, from
     subset.trans H1 H2,
-    show erase (insert e (x ∩ z)) g ⊆ x, by { rw [subset_iff],
+    show (insert e (x ∩ z)).erase g ⊆ x, by { rw [subset_iff],
       intros gg hgg,
       simp only [mem_insert, mem_erase, mem_inter] at hgg,
       rcases hgg.2 with gge | ggxggz,
       { exact gge.symm ▸ he.1, },
-      { exact ggxggz.1, } },
-    show Cg ⊆ erase (insert e (x ∩ z)) g, by
+      { exact ggxggz.1, }, },
+    show Cg ⊆ (insert e (x ∩ z)).erase g, by
       { rw [subset_iff],
       intros gg hgg,
       replace HCg2 : gg ∈ T g := HCg2 hgg,
@@ -659,16 +420,19 @@ begin
         simp only [not_and, mem_sdiff, not_not, mem_inter] at H,
         rcases HCg2.2 with gge | ggz,
         { exact or.inl gge, },
-        { exact or.inr ⟨H hgg ggz, ggz⟩, } } } },
+        { exact or.inr ⟨H hgg ggz, ggz⟩, }, }, }, },
   clear HCg2 he hx,
-  rcases (exists_mem_of_ne_empty HCgzx) with ⟨h0, hh0⟩, clear HCgzx,
+  -- therefore there is an element `h0` in `Cg ∩ (z \ x)`
+  rcases HCgzx with ⟨h0, hh0⟩,
   rw [mem_inter] at hh0,
+  -- let `Ch0` be the circuit contained in `T h0`
   rcases (hTfC h0 hh0.2) with ⟨Ch0, ⟨hCh0circ, hCh0T⟩⟩, clear hTfC,
   have hCgneCh0 : Cg ≠ Ch0 :=
     λ H, have hh0Ch0 : h0 ∉ Ch0 := λ HH, (mem_erase.mp $
       mem_of_subset hCh0T HH).1 rfl, (H.symm ▸ hh0Ch0) hh0.1,
   have hCh0sub : Ch0 ⊆ insert e z :=
-    subset.trans hCh0T (erase_subset h0 $ insert e z),
+    subset.trans hCh0T ((insert e z).erase_subset h0),
+  -- now `e ∈ Cg ∩ Ch0`
   have heCgCh0 : e ∈ Cg ∩ Ch0 :=
     by { rw mem_inter, split,
       { by_contra heCg, have hCgz : Cg ⊆ z :=
@@ -676,9 +440,11 @@ begin
         exact hz.1 Cg HCg1 hCgz },
       { by_contra heCh0, have hCh0z : Ch0 ⊆ z :=
           (erase_eq_of_not_mem heCh0) ▸ (subset_insert_iff.1 hCh0sub),
-        exact hz.1 Ch0 hCh0circ hCh0z } },
+        exact hz.1 Ch0 hCh0circ hCh0z }, },
+  -- so C3 implies that there is a member `CC` of `C.circuits` such that `CC ⊆ (Cg ∪ Ch0).erase e`
   rcases (C.circuit_elim HCg1 hCh0circ hCgneCh0 heCgCh0) with ⟨CC, ⟨hCCcirc, hCCCguCh0⟩⟩,
   clear HCg1 hCh0circ hCgneCh0 heCgCh0,
+  -- both `Cg` and `Ch0` are subsets of `insert e z`, so `CC ⊆ z`,
   have hCCz : CC ⊆ z :=
     by { rw [subset_iff],
     intros t ht,
@@ -689,32 +455,40 @@ begin
     rcases htCguCh0.2 with htCg | htCh0,
     { rcases (mem_insert.mp $ hCgsub htCg) with Hte | Htz,
       { exfalso, exact htCguCh0.1 Hte, },
-      { exact Htz, } },
+      { exact Htz, }, },
     { rcases (mem_insert.mp $ hCh0sub htCh0) with Hte | Htz,
       { exfalso, exact htCguCh0.1 Hte },
-      { exact Htz, } } },
+      { exact Htz, }, }, },
+  -- which is a contradiction; we conclude that I3 holds.
   exact hz.1 CC hCCcirc hCCz,
 end
 
-def indep (C : of_circuits E) : of_indep E :=
-{ indep := C.indep_indep,
+def to_indep (C : of_circuits E) : of_indep E :=
+{ indep := C.indep,
   empty_mem_indep := mem_filter.mpr
     ⟨empty_mem_powerset univ, λ c hc H, C.empty_not_mem_circuits $ (subset_empty.mp H) ▸ hc⟩,
-  indep_of_subset_indep := C.I2,
-  indep_exch := C.I3 }
+  indep_of_subset_indep := I2 C,
+  indep_exch := I3 C, }
 
-/- Not sure if these instances are a good idea... -/
--- instance circ_indep : has_coe (circuits E) (indep E) := ⟨indep_of_circuits⟩
--- instance indep_circ : has_coe (indep E) (circuits E) := ⟨circuits_of_indep⟩
-
-/-- third part of Theorem 1.1.4 -/
-theorem circ_indep_circ : ∀ C : of_circuits E, C = C.indep.circuits
+/-- third part of Theorem 1.1.4: Let `E` be a set and `C` be a collection of subsets
+of `E` satisfying C1-C3. Let `I` be the collection of subsets of `E` that contain
+no member of `C`. Then `(E,I)` has `C` as its collection of circuits. -/
+theorem circ_indep_circ : ∀ C : of_circuits E, C.to_indep.to_circuits = C
   | ⟨c₁, p₁, q₁, r₁⟩ :=
 begin
-  simp only [of_circuits.indep, of_indep.circuits, indep_indep,
-  circuits_circuits, is_circuit, ext, mem_filter, mem_powerset, and_imp, not_and],
+  simp only [to_indep, to_circuits, of_circuits.indep,
+  of_indep.circuits, is_circuit, ext, mem_filter, mem_powerset, and_imp, not_and],
   intro c,
   split,
+  { rintro ⟨hc, ⟨Hc1, Hc2⟩⟩,
+    have : ∃ c' ∈ c₁, c' ⊆ c := by { have := not_forall.mp (Hc1 hc),
+    simpa only [exists_prop, not_forall_not], },
+    rcases this with ⟨c', ⟨hc', hcc'⟩⟩,
+    by_cases h : c = c',
+    { exact h.symm ▸ hc' },
+    { have hc'lt : c' ⊂ c := lt_of_le_of_ne (le_iff_subset.mpr hcc') (ne.symm h),
+      have : c' ∉ c₁ := mt ((Hc2 c' hc'lt).2 c') (not_not.mpr $ subset.refl c'),
+      exact (this hc').elim, }, },
   { intro hc,
     have ce : c ⊆ univ := subset_univ c,
     simp only [ce, true_and, forall_prop_of_true, not_forall, not_not],
@@ -725,16 +499,7 @@ begin
       { intros g hg H,
         have Hc : g < c := lt_of_le_of_lt (le_iff_subset.mpr H) (lt_iff_ssubset.mpr hf),
         have r : g = c := q₁ hg hc (le_of_lt Hc),
-        exact (not_le_of_lt Hc) (le_of_eq r.symm), } } },
-  { rintro ⟨hc, ⟨Hc1, Hc2⟩⟩,
-    have : ∃ c' ∈ c₁, c' ⊆ c := by { have := not_forall.mp (Hc1 hc),
-    simpa only [exists_prop, not_forall_not] },
-    rcases this with ⟨c', ⟨hc', hcc'⟩⟩,
-    by_cases h : c = c',
-    { exact h.symm ▸ hc' },
-    { have hc'lt : c' ⊂ c := lt_of_le_of_ne (le_iff_subset.mpr hcc') (ne.symm h),
-      have : c' ∉ c₁ := mt ((Hc2 c' hc'lt).2 c') (not_not.mpr $ subset.refl c'),
-      exact (this hc').elim, } },
+        exact (not_le_of_lt Hc) (le_of_eq r.symm), }, }, },
 end
 
 end of_circuits
@@ -743,10 +508,13 @@ namespace of_indep
 open of_circuits
 variable {E}
 
-theorem indep_circ_indep (M : of_indep E) : M = M.circuits.indep :=
-suffices M.indep = M.circuits.indep.indep, from eq_of_indep_eq this,
+/-- Let `M` be an independent set matroid and let `C` be `M.to_circuits`,
+its circuit matroid. Then `C.to_indep`, its independent set matroid, is equal to
+`M`. -/
+theorem indep_circ_indep (M : of_indep E) : M.to_circuits.to_indep = M :=
+suffices M.to_circuits.to_indep.indep = M.indep, from eq_of_indep_eq this,
 begin
-  simp only [of_indep.circuits, of_circuits.indep, circuits_circuits, indep_indep,
+  simp only [to_circuits, to_indep, of_indep.circuits, of_circuits.indep,
     ext, mem_powerset, and_imp, mem_filter],
   intro I,
   have hI : I ∈ M.indep → I ⊆ univ := λ H, subset_univ I,
@@ -754,28 +522,42 @@ begin
   intro hIE, have := not_iff_not_of_iff (dep_iff_circuit_subset I M),
   simp only [not_exists, exists_prop, not_and, not_not] at this,
   rw [this, forall_congr],
-  exact λ a, ⟨λ h h₁ h₂ h₃, (h h₃) h₂, λ h h₁ h₂, h (subset.trans h₁ hIE) h₂ h₁⟩,
+  intro a, split,
+  { intros h h₁ h₂, exact h (subset.trans h₁ hIE) h₂ h₁, },
+  { intros h h₁ h₂ h₃, exact (h h₃) h₂, },
 end
 
-/-- Proposition 1.1.6 -/
+/-- the independent set matroids and circuit matroids on a ground set `E` are
+equivalent (there are mutually inverse functions between them) -/
+def indep_equiv_circ : of_indep E ≃ of_circuits E :=
+{ to_fun := to_circuits,
+  inv_fun := to_indep,
+  left_inv := indep_circ_indep,
+  right_inv := circ_indep_circ, }
+
+/-- Proposition 1.1.6: Suppose that `I` is an independent set in a matroid `m` and
+`e` is an element of `m` such that `I ∪ e` is dependent. Then `M` has a unique
+circuit contained in `I ∪ e` and this circuit contains `e`. -/
 theorem existsu_circuit_of_dep_of_insert {I : finset E} {e : E} {m : of_indep E}
   (hI : I ∈ m.indep) (hIe : insert e I ∉ m.indep) :
-  ∃ c, c ∈ m.circuits_circuits ∧ c ⊆ insert e I ∧ e ∈ c ∧
-  ∀ c', c' ∈ m.circuits_circuits → c' ⊆ insert e I → c' = c :=
+  ∃ c, c ∈ m.circuits ∧ c ⊆ insert e I ∧ e ∈ c ∧
+  ∀ c', c' ∈ m.circuits → c' ⊆ insert e I → c' = c :=
 begin
-  simp only [circuits_circuits, mem_powerset, and_imp, mem_filter],
+  simp only [circuits, mem_powerset, and_imp, mem_filter],
   have hIE : I ⊆ univ, from subset_univ I,
   have hc : ∃ (y : finset E) (H : y ⊆ insert e I), is_circuit y m,
     from (dep_iff_circuit_subset (insert e I) m).mp hIe, clear hIe,
+  -- evidently `insert e I` contains a circuit `c`
   rcases hc with ⟨c, ⟨hceI, hccirc⟩⟩,
   have hcE : c ⊆ univ := subset_univ c,
+  -- moreover, every circuit contained in `insert e I` must contain `e`
   have hecirc : ∀ c' ⊆ insert e I, is_circuit c' m → e ∈ c' :=
     by { intros c' hc'eI hc'circ,
       have h₁ := subset_insert_iff.mp hc'eI,
       by_contra h,
       have h₂ := (erase_eq_of_not_mem h).symm,
       have h₃ : c' ⊆ I := calc
-      c' = erase c' e : h₂
+      c' = c'.erase e : h₂
       ... ⊆ I : h₁,
       refine (dep_iff_circuit_subset I m).mpr _ hI,
       use [c', h₃], exact hc'circ, },
@@ -783,21 +565,27 @@ begin
   use c,
   split, { exact ⟨hcE, hccirc⟩, }, { split, { exact hceI, }, { split, { exact hec, },
   { intros c' hc'E hc'circ hc'eI,
+  -- if `c'` is such a circuit
   have hec' : e ∈ c' := hecirc c' hc'eI hc'circ,
-  have hcuc'eI : erase (c ∪ c') e ⊆ I :=
+  -- we have `(c ∪ c').erase e ⊆ I`
+  have hcuc'eI : (c ∪ c').erase e ⊆ I :=
     by { simp only [subset_iff, and_imp, mem_union, mem_insert, mem_erase, ne.def]
       at hceI hc'eI ⊢,
       rintros a hane (H | H),
-      { rcases (hceI H) with H' | H', { exact (hane H').elim, }, { exact H', } },
-      { rcases (hc'eI H) with H' | H', { exact (hane H').elim ,}, { exact H', } } },
-  have : erase (c ∪ c') e ∈ m.indep := m.indep_of_subset_indep hI hcuc'eI,
+      { rcases (hceI H) with H' | H', { exact (hane H').elim, }, { exact H', }, },
+      { rcases (hc'eI H) with H' | H', { exact (hane H').elim ,}, { exact H', }, }, },
+  have : (c ∪ c').erase e ∈ m.indep := m.indep_of_subset_indep hI hcuc'eI,
+  -- and `c'` is distinct from `c`
   by_contra h,
-  have C3 := m.C3 c c' e,
-    simp only [circuits_circuits, mem_powerset, and_imp,
+  -- then by C3,
+  have C3 := m.to_circuits.circuit_elim,
+    simp only [to_circuits, circuits, mem_powerset, and_imp,
       filter_congr_decidable, mem_filter, mem_inter] at C3,
+  -- `(c ∪ c').erase e` contains a circuit `c₀`
   rcases (C3 hcE hccirc hc'E hc'circ (ne.symm h) hec hec') with ⟨c₀, ⟨⟨hc₀, hc₀circ⟩, hc₀erase⟩⟩,
+  -- this is a contradiction, since we just showed this was in `I`.
   refine (dep_iff_circuit_subset I m).mpr _ hI,
-  use [c₀, subset.trans hc₀erase hcuc'eI], exact hc₀circ, } } },
+  use [c₀, subset.trans hc₀erase hcuc'eI], exact hc₀circ, }, }, },
 end
 
 section encodable
@@ -811,8 +599,8 @@ local notation `cdii` := circuit_of_dep_of_insert_indep
 
 lemma circuit_of_dep_of_insert_indep_spec {I : finset E} {e : E} {m : of_indep E}
   (hI : I ∈ m.indep) (hIe : insert e I ∉ m.indep) :
-  cdii hI hIe ∈ m.circuits_circuits ∧ cdii hI hIe ⊆ insert e I ∧
-  e ∈ cdii hI hIe ∧ ∀ c', c' ∈ m.circuits_circuits →
+  cdii hI hIe ∈ m.circuits ∧ cdii hI hIe ⊆ insert e I ∧
+  e ∈ cdii hI hIe ∧ ∀ c', c' ∈ m.circuits →
   c' ⊆ insert e I → c' = cdii hI hIe :=
 encodable.choose_spec (existsu_circuit_of_dep_of_insert hI hIe)
 
@@ -820,19 +608,23 @@ end encodable
 
 end of_indep
 
--- § 1.2
+/-! § 1.2. Bases
+ -/
 
 namespace of_indep
 variable {E}
 
+/-- an independent set is a basis if it is maximal, i.e. all sets strictly
+containing it are dependent. -/
 def is_basis (x : finset E) (m : of_indep E) : Prop :=
 x ∈ m.indep ∧ (∀ y, x ⊂ y → y ∉ m.indep)
 
+/-- the property of being a basis is decidable -/
 instance decidable_basis (x : finset E) (m : of_indep E) : decidable (is_basis x m) :=
 decidable_of_iff (x ∈ m.indep ∧ (∀ y, x ⊂ y → y ∉ m.indep)) $
   by simp only [is_basis, iff_self, finset.mem_powerset]
 
-/-- Lemma 1.2.1 -/
+/-- Lemma 1.2.1. If `x` and `y` are bases of a matroid `m`, then `x.card = y.card` -/
 theorem bases_of_indep_card_eq {x y : finset E} {m : of_indep E} : is_basis x m → is_basis y m →
   card x = card y :=
 begin
@@ -840,18 +632,18 @@ begin
   by_contra heq,
   wlog h : card x < card y using [x y, y x],
   { exact lt_or_gt_of_ne heq, },
-  unfold is_basis at hx hy,
   rcases (m.indep_exch hx.1 hy.1 h) with ⟨e, ⟨he1, he2⟩⟩,
   have hememx : e ∉ x := (mem_sdiff.mp he1).2,
   exact (hx.2 (insert e x) $ ssubset_insert hememx) he2,
 end
 
+/-- every independent set can be extended to a basis -/
 theorem exists_basis_containing_indep {I : finset E} {m : of_indep E} (h : I ∈ m.indep) :
   ∃ B : finset E, I ⊆ B ∧ is_basis B m :=
 begin
-  let F := (m.indep).filter (λ a, I ⊆ a),
+  let F : finset (finset E) := m.indep.filter (λ a, I ⊆ a),
   have FI : I ∈ F := mem_filter.mpr ⟨h, subset.refl I⟩,
-  rcases (max_fun_of_ne_empty card $ ne_empty_of_mem FI) with ⟨B, ⟨HBF, Hg⟩⟩,
+  rcases (max_fun_of_nonempty card $ nonempty_of_mem FI) with ⟨B, ⟨HBF, Hg⟩⟩,
   rw mem_filter at HBF,
   have hBB : is_basis B m := ⟨HBF.1, λ y hBy hyI,
     have hxsy : I ⊆ y := le_of_lt $ lt_of_le_of_lt (le_iff_subset.mpr HBF.2) $
@@ -865,6 +657,8 @@ section encodable
 
 variable [encodable E]
 
+/-- if the ground set is encodable, we can construct a basis containing an
+independent set -/
 def basis_containing_indep {I : finset E} {m : of_indep E} (h : I ∈ m.indep) :
   finset E :=
 encodable.choose $ exists_basis_containing_indep h
@@ -877,6 +671,7 @@ encodable.choose_spec $ exists_basis_containing_indep h
 
 end encodable
 
+/-- any subset with cardinality greater than that of a basis is dependent -/
 theorem dep_of_card_gt_card_basis {x B : finset E} {m : of_indep E} (hB : is_basis B m)
   (hcard : card B < card x) : x ∉ m.indep :=
 begin
@@ -886,6 +681,8 @@ begin
   exact bases_of_indep_card_eq hB hB'basis,
 end
 
+/-- the cardinality of any independent set is less than or equal to that of any
+basis -/
 theorem card_of_indep_le_card_basis {x B : finset E} {m : of_indep E} (hx : x ∈ m.indep)
   (hB : is_basis B m) : card x ≤ card B :=
 begin
@@ -896,24 +693,32 @@ end
 end of_indep
 
 variable (E)
+/-- `of_bases E` is the type of matroids in the basis representation on the ground set
+`E` (encoded in Lean as a `fintype`).
 
+It has the following fields:
+- `bases : finset (finset E)`: the set of bases
+- `bases_not_empty`: axiom (B1), the set of bases is nonempty
+- `basis_exch`: axiom (B2), a basis exchange axiom. If `x` and `y` are bases and
+  `e ∈ x \ y` then there exists an element `a ∈ y \ x` such that `insert a (x.erase e)`
+  is a basis.
+-/
 structure of_bases :=
 (bases : finset (finset E))
 -- (B1)
-(bases_not_empty : bases ≠ ∅)
+(bases_not_empty : bases.nonempty)
 -- (B2)
-(basis_exch {x y e} (hx : x ∈ bases) (hy : y ∈ bases) (he : e ∈ x \ y)
-    : ∃ a, a ∈ y \ x ∧ insert a (erase x e) ∈ bases)
---attribute [class] bases
+(basis_exch {x y : finset E} {e : E} (hx : x ∈ bases) (hy : y ∈ bases) (he : e ∈ x \ y)
+  : ∃ a, a ∈ y \ x ∧ insert a (x.erase e) ∈ bases)
 
 namespace of_bases
-
+/-- a basis matroid is printed by printing its bases -/
 instance bases_repr [has_repr E] : has_repr (of_bases E) :=
 ⟨λ b, has_repr.repr b.bases⟩
 
 variable {E}
-
-theorem eq_of_base_eq : ∀ {B₁ B₂ : of_bases E}, B₁.1 = B₂.1 → B₁ = B₂
+/-- two basis matroids are equal if their bases are equal -/
+lemma eq_of_base_eq : ∀ {B₁ B₂ : of_bases E}, B₁.1 = B₂.1 → B₁ = B₂
   | ⟨b₁, p₁, q₁⟩ ⟨b₂, p₂, q₂⟩ h :=
 by simpa only []
 
@@ -923,54 +728,66 @@ namespace of_indep
 
 variable {E}
 
-def bases_bases (m : of_indep E) : finset (finset E) :=
-(powerset univ).filter (λ S, is_basis S m)
+/-- the set of all bases of an independent set matroid -/
+def bases (m : of_indep E) : finset (finset E) :=
+univ.powerset.filter (λ S, is_basis S m)
 
-lemma B1 (m : of_indep E) : m.bases_bases ≠ ∅ :=
+/-- if `m` is a matroid and `m.bases` its set of bases, then "by (I1)",
+the set of bases is nonempty -/
+private lemma B1 (m : of_indep E) : m.bases.nonempty :=
 begin
-  simp only [is_basis, bases_bases, ext, ne.def, mem_filter, mem_powerset,
-    not_mem_empty, not_and, iff_false],
-  intro h,
-  rcases max_fun_of_ne_empty card (ne_empty_of_mem m.empty_mem_indep) with ⟨a, ⟨ha1, hg⟩⟩,
-  refine (h a (subset_univ a) ha1) _,
+  rcases max_fun_of_nonempty card (nonempty_of_mem m.empty_mem_indep)
+    with ⟨a, ⟨ha1, hg⟩⟩,
+  use a,
+  simp only [bases, mem_filter, mem_powerset, not_and, iff_false,
+    subset_univ, true_and, is_basis, ha1],
   intros F Fcontainsa Findep,
   refine not_le_of_lt (card_lt_card Fcontainsa) _,
   exact hg F Findep,
 end
 
-/- Lemma 1.2.2 -/
-lemma B2 (m : of_indep E) : ∀ (x y : finset E) (e : E), x ∈ m.bases_bases →
-  y ∈ m.bases_bases → e ∈ x \ y →
-  ∃ a, a ∈ y \ x ∧ insert a (erase x e) ∈ m.bases_bases :=
+/- Lemma 1.2.2. If `x` and `y` are members of `m.bases` and `e ∈ x \ y` then
+there is an element `a` of `y \ x` such that `insert a (x.erase e) ∈ m.bases` -/
+private lemma B2 (m : of_indep E) : ∀ (x y : finset E) (e : E), x ∈ m.bases →
+  y ∈ m.bases → e ∈ x \ y →
+  ∃ a, a ∈ y \ x ∧ insert a (x.erase e) ∈ m.bases :=
 begin
-  simp only [is_basis, bases_bases, filter_and, mem_filter, mem_sdiff,
-  mem_powerset, and_imp],
-  intros x y e hxE hxI hx hyE hyI hy hex hey,
-  have hxr : erase x e ∈ m.indep := m.indep_of_subset_indep hxI (erase_subset e x),
-  have hxB : is_basis x m := ⟨hxI, hx⟩, have hyB : is_basis y m := ⟨hyI, hy⟩,
-  have hcard : card (erase x e) < card y := calc
-    card (erase x e) < card x : card_lt_card $ erase_ssubset hex
-    ... = card y : bases_of_indep_card_eq hxB hyB,
-  rcases (m.indep_exch hxr hyI hcard) with ⟨a, ha⟩,
-  clear hxr hyI hcard hyB,
+  simp only [bases, filter_and, mem_filter, mem_sdiff,
+    mem_powerset, and_imp],
+  intros x y e hxE hxB hyE hyB hex hey, clear hxE hyE,
+  -- both `x.erase e` and `y` are independent sets
+  have hxr : x.erase e ∈ m.indep := m.indep_of_subset_indep hxB.1 (erase_subset e x),
+  -- moreover, `(x.erase e).card < y.card`,
+  have hcard : (x.erase e).card < y.card := calc
+    (x.erase e).card < x.card : card_lt_card $ erase_ssubset hex
+    --  since by Lemma 1.2.1 (bases_of_indep_card_eq) `x.card = y.card`
+    ... = y.card : bases_of_indep_card_eq hxB hyB,
+  -- therefore by (I3), there is an element `a` of `y \ (x.erase e)`
+  -- such that `insert a (x.erase e)` is independent
+  rcases (m.indep_exch hxr hyB.1 hcard) with ⟨a, ha⟩,
+  clear hxr hcard hyB,
   have ha1 := mem_sdiff.mp ha.1,
+  -- since `a ≠ e` and `a ∉ x`
   have hae : a ≠ e := λ hae, hey $ hae ▸ ha1.1,
   have hax : a ∉ x := by { simp only [not_and, mem_erase, ne.def] at ha1, exact ha1.2 hae },
-  have hcx : card x > 0 := card_pos.mpr (ne_empty_of_mem hex),
-  have hayycard : card (insert a $ erase x e) = card x := calc
-    card (insert a $ erase x e) = nat.pred (card x) + 1 : by rw [card_insert_of_not_mem ha1.2,
+  have hcx : x.card > 0 := card_pos.mpr (nonempty_of_mem hex),
+  -- `insert a (x.erase e)` is the same size as `x`
+  have hayycard : (insert a $ x.erase e).card = x.card := calc
+    (insert a $ x.erase e).card = x.card.pred + 1 : by rw [card_insert_of_not_mem ha1.2,
         card_erase_of_mem hex]
-    ... = card x : nat.succ_pred_eq_of_pos hcx,
-  use a, simp only [ha1.1, hax, true_and, not_false_iff, ha.2, subset_univ],
+    ... = x.card : nat.succ_pred_eq_of_pos hcx,
+  -- hence `insert a (x.erase e)` is a basis
+  use a, simp only [ha1.1, hax, true_and, not_false_iff, ha.2, subset_univ, is_basis],
   intros y' hayy,
   refine dep_of_card_gt_card_basis hxB _,
   exact hayycard ▸ (card_lt_card hayy),
 end
 
-def bases (m : of_indep E) : of_bases E :=
-{ bases := bases_bases m,
-  bases_not_empty := m.B1,
-  basis_exch := m.B2 }
+/-- `m.to_bases` is the basis matroid corresponding to the independent set matroid `m` -/
+def to_bases (m : of_indep E) : of_bases E :=
+{ bases := bases m,
+  bases_not_empty := B1 m,
+  basis_exch := B2 m }
 
 end of_indep
 
@@ -978,162 +795,241 @@ namespace of_bases
 open of_indep
 variable {E}
 
-/-- Lemma 1.2.4 -/
+/-- Lemma 1.2.4. The bases of a basis matroid  are equicardinal. -/
 theorem bases_card_eq {x y : finset E} {b : of_bases E} (hx : x ∈ b.bases) (hy : y ∈ b.bases) :
-  card x = card y :=
+  x.card = y.card :=
 begin
+  -- suppose `x` and `y` are distinct bases with `y.card < x.card`
   by_contra heq,
-  wlog h : card y < card x using [x y, y x],
-  exact lt_or_gt_of_ne (ne.symm heq), clear heq,
-  let F : finset (finset E × finset E) := (finset.product b.bases b.bases).filter
+  wlog h : y.card < x.card using [x y, y x],
+  { exact lt_or_gt_of_ne (ne.symm heq), }, clear heq,
+  -- let `F` be the set of all such pairs
+  let F : finset (finset E × finset E) := (b.bases.product b.bases).filter
     (λ e : finset E × finset E, card e.1 < card e.2),
+  -- `F` is nonempty
   have hyx : (y, x) ∈ F := mem_filter.mpr ⟨mem_product.mpr ⟨hy, hx⟩, h⟩, clear hy hx,
-  exact exists.elim (min_fun_of_ne_empty (λ f : finset E × finset E, card (f.2 \ f.1)) $
-      ne_empty_of_mem hyx)
-    (λ a ha, exists.elim ha $ by { clear hyx ha,
-      intros haF Ha, replace haF := mem_filter.mp haF,
-      have hab : a.1 ∈ b.bases ∧ a.2 ∈ b.bases := mem_product.mp haF.1,
-      exact exists.elim (exists_sdiff_of_card_lt haF.2)
-        (λ e he, exists.elim (b.basis_exch hab.2 hab.1 he) $ λ aa ⟨haa1, haa2⟩,
-          by { rw mem_sdiff at haa1,
-          let a2 : finset E := insert aa (erase a.2 e),
-          have haani : aa ∉ erase a.2 e := λ h, haa1.2 (mem_erase.mp h).2,
-          have hea2 : e ∈ a.2 := (mem_sdiff.mp he).1,
-          have hpos : 0 < card a.2 := card_pos.mpr (ne_empty_of_mem hea2),
-          have hcarda2 : card a.1 < card a2 := by { rw [card_insert_of_not_mem haani,
-            card_erase_of_mem hea2, ←nat.succ_eq_add_one, nat.succ_pred_eq_of_pos hpos],
-            exact haF.2 }, clear haani hpos,
-          have : e ∉ a2 := λ hh, or.elim (mem_insert.mp hh)
-            (λ h4, haa1.2 $ h4 ▸ hea2) $ λ h5, (mem_erase.mp h5).1 rfl,
-          have hcard : card (a2 \ a.1) < card (a.2 \ a.1) :=
-            suffices a2 \ a.1 ⊂ a.2 \ a.1, from card_lt_card this,
-            by { rw ssubset_iff,
-            exact exists.intro e ⟨λ h0, this (mem_sdiff.mp h0).1,
-              by { rw subset_iff,
-              intros A hA, rw mem_insert at hA,
-              exact or.elim hA (λ hA1, hA1.symm ▸ he)
-                (by { intro hA2, rw [mem_sdiff, mem_insert] at hA2,
-                exact mem_sdiff.mpr ⟨or.elim hA2.1 (λ h6, false.elim $ hA2.2 $ h6.symm ▸ haa1.1) $
-                  λ h7, (mem_erase.mp h7).2, hA2.2⟩ }) }⟩ },
-          have ha2F : (a.1, a2) ∈ F := mem_filter.mpr ⟨mem_product.mpr ⟨hab.1, haa2⟩, hcarda2⟩,
-          exact not_le_of_lt hcard (Ha (a.1, a2) ha2F) }) })
+  -- so we may select a pair `a` = `(a.1, a.2)` such that `(a.2 \ a.1).card` is minimal
+  rcases (min_fun_of_nonempty (λ f : finset E × finset E, (f.2 \ f.1).card) $
+      nonempty_of_mem hyx) with ⟨a, haF, Ha⟩,
+  clear hyx,
+  replace haF := mem_filter.mp haF,
+  have hab : a.1 ∈ b.bases ∧ a.2 ∈ b.bases := mem_product.mp haF.1,
+  -- clearly `a.2 \ a.1` is nonempty, so choose `e` in `a.2 \ a.1`
+  rcases (nonempty_sdiff_of_card_lt haF.2) with ⟨e, he⟩,
+  -- we can find an element `aa` of `a.1 \ a.2` so that `insert aa (a.2.erase e)` is a basis
+  rcases (b.basis_exch hab.2 hab.1 he) with ⟨aa, haa1, haa2⟩,
+  rw mem_sdiff at haa1,
+  -- from now on we call `insert aa (a.2.erase e)` `a2`
+  let a2 : finset E := insert aa (a.2.erase e),
+  have haani : aa ∉ a.2.erase e := λ h, haa1.2 (mem_erase.mp h).2,
+  have hea2 : e ∈ a.2 := (mem_sdiff.mp he).1,
+  have hpos : 0 < a.2.card := card_pos.mpr (nonempty_of_mem hea2),
+  -- evidently `a2.card > a.1.card`
+  have hcarda2 : a.1.card < a2.card := by { rw [card_insert_of_not_mem haani,
+    card_erase_of_mem hea2, ←nat.succ_eq_add_one, nat.succ_pred_eq_of_pos hpos],
+    exact haF.2 }, clear haani hpos haF,
+  have : e ∉ a2 := by { intro hh,
+    rcases mem_insert.mp hh with rfl | hh,
+    { exact haa1.2 hea2, },
+    { rw mem_erase at hh, exact hh.1 rfl, }, }, clear hea2,
+  -- and `(a2 \ a.1).card < (a.2 \ a.1).card`
+  have hcard : (a2 \ a.1).card < (a.2 \ a.1).card :=
+    suffices a2 \ a.1 ⊂ a.2 \ a.1, from card_lt_card this,
+    by { rw ssubset_iff,
+      use e,
+      split,
+      { intro h0, exact this (mem_sdiff.mp h0).1, },
+      { rw subset_iff,
+        intros A hA, rw mem_insert at hA,
+        rcases hA with rfl | hA,
+        { exact he, },
+        { rw [mem_sdiff, mem_insert] at hA,
+        refine mem_sdiff.mpr ⟨_, hA.2⟩,
+        rcases hA.1 with rfl | hA,
+        { simp only [true_and, true_or, mem_erase, eq_self_iff_true A] at hA,
+          exfalso, exact hA haa1.1, },
+        { exact (mem_erase.mp hA).2, }, }, }, }, clear he haa1 this,
+  -- thus the choice of `a.1` and `a.2` is contradicted
+  have ha2F : (a.1, a2) ∈ F := mem_filter.mpr ⟨mem_product.mpr ⟨hab.1, haa2⟩, hcarda2⟩,
+  -- and the lemma is proved
+  exact not_le_of_lt hcard (Ha (a.1, a2) ha2F)
 end
 
-def indep_indep (b : of_bases E) : finset (finset E) :=
-(powerset univ).filter (λ x, ∃ a ∈ b.bases, x ⊆ a)
+/-- `b.indep` for `b` a basis matroid (type `of_bases E`) is the set of
+all independent sets of `E`, i.e. all sets contained in elements of `b.bases` -/
+def indep (b : of_bases E) : finset (finset E) :=
+univ.powerset.filter (λ x, ∃ a ∈ b.bases, x ⊆ a)
 
-/-- first part of Theorem 1.2.3 -/
-def indep (b : of_bases E) : of_indep E :=
-{ indep := b.indep_indep,
-  empty_mem_indep := mem_filter.mpr ⟨empty_mem_powerset univ,
-    exists.elim (exists_mem_of_ne_empty b.bases_not_empty) $
-      λ a ha, exists.intro a $ exists.intro ha $ empty_subset a⟩,
+/-- Part I3 of Lemma 1.2.3. Let `E` be a set and `b` be a basis matroid on `E`. Let
+`b.indep` be the collection of subsets of `E` contained in some member of `b.bases`.
+Then `b.indep` satisfies axiom I3. (For any two elements of `b.indep`, `x`, `y` with
+`x.card < y.card`, there exists an element `e ∈ y \ x` such that
+`insert e x ∈ b.indep`.) -/
+private lemma I3 (b : of_bases E) (x y : finset E) (hx : x ∈ b.indep)
+  (hy : y ∈ b.indep) (hcard : x.card < y.card)
+  : ∃ e, e ∈ y \ x ∧ insert e x ∈ b.indep :=
+begin
+  unfold indep at hx hy ⊢,
+  let F := b.bases.filter (λ S, S ⊆ y),
+  -- suppose that I3 fails for `b.indep`, then
+  by_contra h,
+  -- `x` and `y` are elements of `b.indep` with `x.card < y.card` such that
+  -- for all `e ∈ y \ x`, the set `insert e x ∉ b.indep`
+  simp only [mem_powerset, not_exists, and_imp, filter_congr_decidable,
+    exists_prop, mem_filter, not_and, mem_sdiff] at hx hy h,
+  -- by definition, `b.bases` contain members `b1` and `b2` such that `x ⊆ b1` and `y ⊆ b2`
+  rcases hx.2 with ⟨b1, ⟨hb1bases, hxb1⟩⟩, clear hx,
+  rcases hy.2 with ⟨b2, hb2⟩, clear hy,
+  -- assume that such a set `B2` is chosen so that `B2 \ (y ∪ b1)` is minimal
+  have := (min_fun_of_nonempty (λ f, (f \ (y ∪ b1)).card) $
+    nonempty_of_mem $ mem_filter.mpr hb2), clear hb2 b2,
+  rcases this with ⟨B2, ⟨hB2filt, hB2min⟩⟩,
+  replace hB2filt : B2 ∈ b.bases ∧ y ⊆ B2 := mem_filter.mp hB2filt,
+  -- by the choice of `x` and `y`, `y \ b1 = y \ x` (1)
+  have hysdiff : y \ b1 = y \ x := by { simp only [ext, mem_sdiff],
+    intro gg,
+    split,
+    { rintros ⟨hggy, hggnb1⟩, split, { exact hggy, },
+      { intro hggnx, exact hggnb1 (mem_of_subset hxb1 hggnx), }, },
+    { rintros ⟨hggy, hggnx⟩, split, { exact hggy, },
+      { intro hggnb1,
+        have : ¬insert gg x ⊆ b1 := h gg hggy hggnx (subset_univ _) b1 hb1bases,
+        exact this (insert_subset.mpr ⟨hggnb1, hxb1⟩), }, }, },
+  have hB2yub1: B2 \ (y ∪ b1) = ∅ := by {
+    -- now suppose `B2 \ (y ∪ b1)` is nonempty
+    by_contra H,
+    -- then we can choose an element `X` from this set
+    rcases (nonempty_of_ne_empty H) with ⟨X, hX⟩, clear H,
+    simp only [not_or_distrib, mem_union, mem_sdiff] at hX,
+    have hXB2b1 : X ∈ B2 \ b1 := by { rw mem_sdiff, exact ⟨hX.1, hX.2.2⟩ },
+    -- by (B2) there is an element `Y` of `b1 \ B2` such that `insert Y (B2.erase X) ∈ b.bases`
+    rcases (b.basis_exch hB2filt.1 hb1bases hXB2b1) with ⟨Y, ⟨hYb1B2, hYbases⟩⟩,
+    rw mem_sdiff at hYb1B2 hXB2b1,
+    -- but then `(insert Y (B2.erase X) \ (y ∪ b1)).card < (B2 \ (y ∪ b1)).card`,
+    -- and the choice of B2 is contradicted
+    have hssubY : insert Y (B2.erase X) \ (y ∪ b1) ⊂ B2 \ (y ∪ b1) :=
+      by { rw [ssubset_iff],
+      use X,
+      simp only [subset_iff, not_or_distrib, mem_union, mem_insert, not_and, mem_sdiff,
+        not_not, mem_erase, not_true, or_false, ne.def, false_and, or_false,
+        eq_self_iff_true],
+      split,
+      { rintro rfl hXy, exact hYb1B2.1, },
+      { rintro gg (rfl | ⟨rfl | ⟨hggnX, hggB2⟩, hggny, hggnb1⟩),
+        { exact hX, },
+        { exact (hggnb1 hYb1B2.1).elim, },
+        { exact ⟨hggB2, hggny, hggnb1⟩, }, }, },
+    replace hssubY := card_lt_card hssubY,
+    have hysubY : y ⊆ insert Y (B2.erase X) := by {
+      simp only [subset_iff, mem_insert, mem_erase, ne.def],
+      exact λ gg hgg, or.inr ⟨λ ggx, hX.2.1 $ ggx ▸ hgg, mem_of_subset hB2filt.2 hgg⟩, },
+    -- hence `B2 \ (y ∪ b1)` is empty
+    exact not_lt_of_le (hB2min (insert Y $ B2.erase X) $ mem_filter.mpr
+        ⟨hYbases, hysubY⟩) hssubY }, clear hB2min,
+  rw [←subset_iff_sdiff_eq_empty, subset_iff] at hB2yub1, simp only [mem_union] at hB2yub1,
+  -- and so `B2 \ b1 = y \ b1`
+  have hB2b1y : B2 \ b1 = y \ b1 := by { simp only [ext, mem_sdiff],
+    exact λ gg, ⟨λ hgg, ⟨(hB2yub1 hgg.1).elim id $ λ hb1, (hgg.2 hb1).elim, hgg.2⟩,
+        λ hgg, ⟨mem_of_subset hB2filt.2 hgg.1, hgg.2⟩⟩ }, clear hB2yub1,
+  -- Thus, by (1), `B2 \ b1 = y \ x`. (2)
+  rw [hysdiff] at hB2b1y, clear hysdiff,
+  -- Next we show that `b1 \ (x ∪ B2)` is empty.
+  have hb1xuB2 : b1 \ (x ∪ B2) = ∅ := by {
+    -- if not,
+    by_contra H,
+    -- then there is an element `X` in this set
+    rcases (nonempty_of_ne_empty H) with ⟨X, hX⟩,
+    simp only [not_or_distrib, mem_union, mem_sdiff] at hX,
+    -- and an element `Y` in `B2 \ b1` so that `insert Y (b1.erase X) ∈ b.bases`.
+    rcases (b.basis_exch hb1bases hB2filt.1 $ mem_sdiff.mpr ⟨hX.1, hX.2.2⟩) with ⟨Y, hY⟩,
+    -- since `Y ∈ B2 \ b1`,
+    rw mem_sdiff at hY,
+    -- it follows by (2) that `Y ∈ y \ x`
+    have hYyx : Y ∈ y ∧ Y ∉ x := mem_sdiff.mp (hB2b1y ▸ (mem_sdiff.mpr hY.1)),
+    -- now `insert Y x ⊆ insert Y (b1.erase X)`,
+    have hxYsub : insert Y x ⊆ insert Y (b1.erase X) := by {
+      simp only [subset_iff, mem_insert, mem_erase, ne.def],
+      exact λ gg hgg, or.elim hgg (λ ggY, or.inl ggY) $ λ ggx, or.inr ⟨λ ggX, hX.2.1 $
+        ggX ▸ ggx, mem_of_subset hxb1 ggx⟩ },
+    -- so `insert Y x ∈ b.indep`
+    -- and so we have a contradiction to our assumption that (I3) fails
+    -- we conclude that `b1 \ (x ∪ B2)` is empty
+    exact h Y hYyx.1 hYyx.2 (subset_univ _) (insert Y $ b1.erase X) hY.2 hxYsub, },
+  clear h,
+  rw [←subset_iff_sdiff_eq_empty, subset_iff] at hb1xuB2, simp only [mem_union] at hb1xuB2,
+  -- Hence `b1 \ B2 = x \ B2`.
+  have hb1B2 : b1 \ B2 = x \ B2 := by { simp only [ext, mem_sdiff],
+    exact λ gg, ⟨λ hgg, ⟨(hb1xuB2 hgg.1).elim id $ λ ggB2, (hgg.2 ggB2).elim, hgg.2⟩,
+        λ hgg, ⟨mem_of_subset hxb1 hgg.1, hgg.2⟩⟩, }, clear hb1xuB2,
+  -- Since the last set is contained in `x \ y` it follows that
+  -- `b1 \ B2 ⊆ x \ y` (3)
+  replace hb1B2 : b1 \ B2 ⊆ x \ y := hb1B2.symm ▸ (sdiff_subset_sdiff (subset.refl x)
+      hB2filt.2),
+  -- By Lemma 1.2.4, `b1.card = B2.card`,
+  have hcardeq : b1.card = B2.card := bases_card_eq hb1bases hB2filt.1,
+  -- so `(b1 \ B2).card = (B2 \ b1).card`.
+  have hcardb1B2 : (b1 \ B2).card = (B2 \ b1).card := calc
+    (b1 \ B2).card = b1.card - (b1 ∩ B2).card : card_sdiff_eq b1 B2
+    ... = B2.card - (B2 ∩ b1).card : by rw [hcardeq, inter_comm]
+    ... = (B2 \ b1).card : by rw ←card_sdiff_eq B2 b1,
+  -- Therefore, by (2) and (3), `(y \ x).ccard ≤ (x \ y).card`,
+  have hcardcontra0 : (y \ x).card ≤ (x \ y).card := calc
+    (y \ x).card = (B2 \ b1).card : by rw hB2b1y
+    ... = (b1 \ B2).card : by rw hcardb1B2
+    ... ≤ (x \ y).card : card_le_of_subset hb1B2,
+  rw [card_sdiff_eq y x, card_sdiff_eq x y, inter_comm] at hcardcontra0,
+  -- so `y.card ≤ x.card`
+  have hcardcontra : y.card ≤ x.card := nat.le_of_le_of_sub_le_sub_right
+      (card_le_of_subset $ inter_subset_left x y) hcardcontra0,
+  -- This contradiction completes the proof of (I3)
+  exact not_lt_of_le hcardcontra hcard,
+end
+
+/-- first part of Theorem 1.2.3; Let `E` be a set and `b` be a basis matroid on `E`. Let
+`b.indep` be the collection of subsets of `E` contained in some member of `b.bases`.
+Then `b.to_indep` is an independent set matroid with type `of_indep E` -/
+def to_indep (b : of_bases E) : of_indep E :=
+{ indep := b.indep,
+  empty_mem_indep := begin
+      refine mem_filter.mpr ⟨empty_mem_powerset univ, _⟩,
+      convert b.bases_not_empty,
+      simp only [exists_prop, finset.empty_subset, and_true],
+    end,
   indep_of_subset_indep := begin
       intros x y hx hxy,
-      simp only [indep_indep, mem_powerset, filter_congr_decidable,
+      simp only [indep, mem_powerset, filter_congr_decidable,
         exists_prop, mem_filter] at hx ⊢,
       split, { exact subset.trans hxy hx.1, },
-      { rcases hx.2 with ⟨a, ha⟩, use a, exact ⟨ha.1, subset.trans hxy ha.2⟩, },
+      { rcases hx.2 with ⟨a, ha1, ha2⟩, use [a, ha1], exact subset.trans hxy ha2, },
     end,
-  indep_exch := begin
-    intros x y hx hy hcard, unfold indep_indep at hx hy ⊢,
-    let F := (b.bases).filter (λ S, S ⊆ y),
-    by_contra h, simp only [mem_powerset, not_exists, and_imp, filter_congr_decidable,
-      exists_prop, mem_filter, not_and, mem_sdiff] at hx hy h,
-    rcases hx.2 with ⟨b1, ⟨hb1bases, hxb1⟩⟩,
-    rcases hy.2 with ⟨b2, hb2⟩,
-    have := (min_fun_of_ne_empty (λ f, card (f \ (y ∪ b1))) $
-      ne_empty_of_mem $ mem_filter.mpr hb2),
-    rcases this with ⟨B2, ⟨hB2filt, hB2min⟩⟩, clear hb2 b2,
-    replace hB2filt : B2 ∈ b.bases ∧ y ⊆ B2 := mem_filter.mp hB2filt,
-    have hysdiff : y \ b1 = y \ x := by { simp only [ext, mem_sdiff],
-      exact λ gg, ⟨λ hgg, ⟨hgg.1, λ hggnx, hgg.2 $ mem_of_subset hxb1 hggnx⟩,
-        λ hgg, ⟨hgg.1, λ ggb1, h gg hgg.1 hgg.2 (insert_subset.mpr
-        ⟨mem_of_subset hy.1 hgg.1, hx.1⟩) b1 hb1bases $ insert_subset.mpr ⟨ggb1, hxb1⟩⟩⟩, },
-    have hB2yub1: B2 \ (y ∪ b1) = ∅ := by { by_contra H,
-      rcases (exists_mem_of_ne_empty H) with ⟨X, hX⟩, clear H,
-      simp only [not_or_distrib, mem_union, mem_sdiff] at hX,
-      have hXB2b1 : X ∈ B2 \ b1 := by { rw mem_sdiff, exact ⟨hX.1, hX.2.2⟩ },
-      rcases (b.basis_exch hB2filt.1 hb1bases hXB2b1) with ⟨Y, ⟨hYb1B2, hYbases⟩⟩,
-      rw mem_sdiff at hYb1B2 hXB2b1,
-      have hssubY : insert Y (erase B2 X) \ (y ∪ b1) ⊂  B2 \ (y ∪ b1) :=
-        by { rw [ssubset_iff],
-        use X,
-        simp only [subset_iff, not_or_distrib, mem_union, mem_insert, not_and, mem_sdiff,
-          not_not, mem_erase, not_true, or_false, ne.def, false_and, or_false,
-          eq_self_iff_true],
-        exact ⟨λ hXY, (hYb1B2.2 $ hXY ▸ hXB2b1.1).elim,
-        λ gg hgg, or.elim hgg (λ ggx, ggx.symm ▸ hX) $ λ ggor2, or.elim ggor2.1
-          (λ ggY, false.elim $ ((ggY ▸ ggor2.2.2) hYb1B2.1)) $
-            λ ggXB2, ⟨ggXB2.2, ggor2.2⟩⟩, },
-      replace hssubY := card_lt_card hssubY,
-      have hysubY : y ⊆ insert Y (erase B2 X) := by {
-        simp only [subset_iff, mem_insert, mem_erase, ne.def],
-        exact λ gg hgg, or.inr ⟨λ ggx, hX.2.1 $ ggx ▸ hgg, mem_of_subset hB2filt.2 hgg⟩ },
-      exact not_lt_of_le (hB2min (insert Y $ erase B2 X) $ mem_filter.mpr
-          ⟨hYbases, hysubY⟩) hssubY }, clear hB2min,
-      rw [←subset_iff_sdiff_eq_empty, subset_iff] at hB2yub1, simp only [mem_union] at hB2yub1,
-      have hB2b1y : B2 \ b1 = y \ b1 := by { simp only [ext, mem_sdiff],
-        exact λ gg, ⟨λ hgg, ⟨or.elim (hB2yub1 hgg.1) id $ λ hb1, false.elim $ hgg.2 hb1, hgg.2⟩,
-            λ hgg, ⟨mem_of_subset hB2filt.2 hgg.1, hgg.2⟩⟩ },
-      rw [hysdiff] at hB2b1y, clear hysdiff,
-      have hb1xuB2 : b1 \ (x ∪ B2) = ∅ := by { by_contra H,
-        rcases (exists_mem_of_ne_empty H) with ⟨X, hX⟩,
-        simp only [not_or_distrib, mem_union, mem_sdiff] at hX,
-        rcases (b.basis_exch hb1bases hB2filt.1 $ mem_sdiff.mpr ⟨hX.1, hX.2.2⟩) with ⟨Y, hY⟩,
-        rw mem_sdiff at hY,
-        have hYyx : Y ∈ y ∧ Y ∉ x := mem_sdiff.mp (hB2b1y ▸ (mem_sdiff.mpr hY.1)),
-        have hxYsub : insert Y x ⊆ insert Y (erase b1 X) := by {
-          simp only [subset_iff, mem_insert, mem_erase, ne.def],
-          exact λ gg hgg, or.elim hgg (λ ggY, or.inl ggY) $ λ ggx, or.inr ⟨λ ggX, hX.2.1 $
-            ggX ▸ ggx, mem_of_subset hxb1 ggx⟩ },
-        exact h Y hYyx.1 hYyx.2 (subset_univ (insert Y x)) (insert Y $ erase b1 X) hY.2 hxYsub, },
-      clear h hx hy,
-      rw [←subset_iff_sdiff_eq_empty, subset_iff] at hb1xuB2, simp only [mem_union] at hb1xuB2,
-      have hb1B2 : b1 \ B2 = x \ B2 := by { simp only [ext, mem_sdiff],
-        exact λ gg, ⟨λ hgg, ⟨or.elim (hb1xuB2 hgg.1) id $ λ ggB2, false.elim $ hgg.2 ggB2, hgg.2⟩,
-            λ hgg, ⟨mem_of_subset hxb1 hgg.1, hgg.2⟩⟩ }, clear hb1xuB2,
-      replace hb1B2 : b1 \ B2 ⊆ x \ y := hb1B2.symm ▸ (sdiff_subset_sdiff (subset.refl x)
-          hB2filt.2),
-      have hcardeq : card b1 = card B2 := bases_card_eq hb1bases hB2filt.1,
-      have hcardb1B2 : card (b1 \ B2) = card (B2 \ b1) := calc
-        card (b1 \ B2) = card b1 - card (b1 ∩ B2) : card_sdiff_eq b1 B2
-        ... = card B2 - card (B2 ∩ b1) : by rw [hcardeq, inter_comm]
-        ... = card (B2 \ b1) : by rw ←card_sdiff_eq B2 b1,
-      have hcardcontra0 : card (y \ x) ≤ card (x \ y) := calc
-        card (y \ x) = card (B2 \ b1) : by rw hB2b1y
-        ... = card (b1 \ B2) : by rw hcardb1B2
-        ... ≤ card (x \ y) : card_le_of_subset hb1B2,
-      rw [card_sdiff_eq y x, card_sdiff_eq x y, inter_comm] at hcardcontra0,
-      have hcardcontra : card y ≤ card x := nat.le_of_le_of_sub_le_sub_right
-          (card_le_of_subset $ inter_subset_left x y) hcardcontra0,
-      exact not_lt_of_le hcardcontra hcard,
-    end }
+  indep_exch := I3 b, }
 
 -- instance base_indep : has_coe (bases E) (indep E) := ⟨indep_of_bases⟩
 -- instance indep_base : has_coe (indep E) (bases E) := ⟨bases_of_indep⟩
 
-/-- second part of Theorem 1.2.3 -/
-theorem base_indep_base (B : of_bases E) : B = B.indep.bases :=
-suffices B.bases = B.indep.bases.bases, from eq_of_base_eq this,
+/-- second part of Theorem 1.2.3, Let `E` be a set and `b` be a basis matroid on `E`. Let
+`b.indep` be the collection of subsets of `E` contained in some member of `b.bases`.
+Then `b.to_indep` has `b.bases` as its set of bases -/
+theorem bases_indep_bases (B : of_bases E) : B.to_indep.to_bases = B :=
+suffices B.to_indep.to_bases.bases = B.bases, from eq_of_base_eq this,
 begin
-  simp only [of_bases.indep, of_indep.bases, indep_indep, is_basis,
-  ext, bases_bases, mem_filter, mem_powerset, not_and, not_exists, exists_prop],
+  simp only [to_indep, to_bases, of_bases.indep, is_basis,
+  ext, of_indep.bases, mem_filter, mem_powerset, not_and, not_exists, exists_prop],
   intro b, split,
-  { intro hb,
-    have hB : b ⊆ univ := subset_univ b,
-    split,
-    { exact hB, },
-    { split, { split, { exact hB, }, { use b, exact ⟨hb, subset.refl b⟩, } },
-      { intros b' hbb' _ _ hx H,
-        exact (ne_of_lt $ lt_of_lt_of_le (card_lt_card hbb') $ card_le_of_subset H)
-          (bases_card_eq hb hx) } } },
   { rintro ⟨_, ⟨⟨_, hbexists⟩, hb⟩⟩, rcases hbexists with ⟨a, ⟨habases, hba⟩⟩,
     have : a ⊆ univ := subset_univ a,
     by_cases h : a = b,
     { exact h ▸ habases, },
     { have hba' : b ⊂ a := lt_iff_ssubset.mp (lt_of_le_of_ne (le_iff_subset.mpr hba) $ ne.symm h),
-      exact (hb a hba' this a habases $ subset.refl a).elim, } },
+      exact (hb a hba' this a habases $ subset.refl a).elim, }, },
+  { intro hb,
+    have hB : b ⊆ univ := subset_univ b,
+    split,
+    { exact hB, },
+    { split, { split, { exact hB, }, { use b, exact ⟨hb, subset.refl b⟩, }, },
+      { intros b' hbb' _ _ hx H,
+        exact (ne_of_lt $ lt_of_lt_of_le (card_lt_card hbb') $ card_le_of_subset H)
+          (bases_card_eq hb hx), }, }, },
 end
 
 end of_bases
@@ -1142,25 +1038,39 @@ namespace of_indep
 open of_bases
 variable {E}
 
-theorem indep_base_indep (M : of_indep E) : M = M.bases.indep :=
-suffices M.indep = M.bases.indep.indep, from eq_of_indep_eq this,
+/-- Let `M` be an independent set matroid and let `B` be `M.to_bases`,
+its corresponding basis matroid. Then `B.to_indep`, its independent set matroid
+is equal to `M`. -/
+theorem indep_bases_indep (M : of_indep E) : M.to_bases.to_indep = M :=
+suffices M.to_bases.to_indep.indep = M.indep, from eq_of_indep_eq this,
 begin
-  simp only [of_bases.indep, of_indep.bases, indep_indep, is_basis,
-  ext, bases_bases, mem_filter, mem_powerset, exists_prop],
+  simp only [to_indep, to_bases, of_bases.indep, is_basis,
+  ext, of_indep.bases, mem_filter, mem_powerset, exists_prop],
   intro I, split,
+  { rintro ⟨hIuniv, hIexists⟩, rcases hIexists with ⟨B, ⟨⟨hBuniv, ⟨hBindep, hB'⟩⟩, hIB⟩⟩,
+    exact M.indep_of_subset_indep hBindep hIB, },
   { intro hI, split,
     { exact subset_univ I, },
     { rcases (exists_basis_containing_indep hI) with ⟨B, hB⟩,
       unfold is_basis at hB,
-      use B, exact ⟨⟨subset_univ B, hB.2⟩, hB.1⟩ } },
-  { rintro ⟨hIuniv, hIexists⟩, rcases hIexists with ⟨B, ⟨⟨hBuniv, ⟨hBindep, hB'⟩⟩, hIB⟩⟩,
-    exact M.indep_of_subset_indep hBindep hIB, },
+      use B, exact ⟨⟨subset_univ B, hB.2⟩, hB.1⟩, }, },
 end
 
-/-- Corollary 1.2.6 -/
+/-- the independent set matroids and basis matroids on a ground set `E` are
+equivalent (there are mutually inverse functions between them) -/
+def indep_equiv_bases : of_indep E ≃ of_bases E :=
+{ to_fun := to_bases,
+  inv_fun := to_indep,
+  left_inv := indep_bases_indep,
+  right_inv := bases_indep_bases, }
+
+/-- Corollary 1.2.6. Let `B` be a basis of a matroid `m`. If
+`e ∈ (univ : finset E) \ B`, then `insert e B` contains a unique circuit `C`.
+Moreover, `e ∈ C`. We call this the fundamental circuit of `e` with respect
+to `B`. -/
 theorem existsu_fund_circ_of_basis {m : of_indep E} {B : finset E} (hB : is_basis B m) {e : E}
-  (he : e ∈ univ \ B) : ∃ C, C ∈ m.circuits_circuits ∧ C ⊆ insert e B ∧
-  ∀ C' ∈ m.circuits_circuits, C' ⊆ insert e B → C' = C :=
+  (he : e ∈ univ \ B) : ∃ C, C ∈ m.circuits ∧ C ⊆ insert e B ∧
+  ∀ C' ∈ m.circuits, C' ⊆ insert e B → C' = C :=
 begin
   unfold is_basis at hB, rw mem_sdiff at he,
   have : insert e B ∉ m.indep := hB.2 (insert e B) (ssubset_insert he.2),
@@ -1173,14 +1083,15 @@ end
 section encodable
 
 variable [encodable E]
-
+/-- The fundamental circuit of a basis (see `existsu_fund_circ_of_basis`)
+can be computed for an encodable ground set. -/
 def fund_circ_of_basis {m : of_indep E} {B : finset E} (hB : is_basis B m) {e : E}
   (he : e ∈ univ \ B) : finset E :=
 encodable.choose (existsu_fund_circ_of_basis hB he)
 
 lemma fund_circ_of_basis_spec {m : of_indep E} {B : finset E} (hB : is_basis B m) {e : E}
-  (he : e ∈ univ \ B) : fund_circ_of_basis hB he ∈ m.circuits_circuits ∧
-  fund_circ_of_basis hB he  ⊆ insert e B ∧ ∀ C' ∈ m.circuits_circuits, C' ⊆ insert e B →
+  (he : e ∈ univ \ B) : fund_circ_of_basis hB he ∈ m.circuits ∧
+  fund_circ_of_basis hB he  ⊆ insert e B ∧ ∀ C' ∈ m.circuits, C' ⊆ insert e B →
   C' = fund_circ_of_basis hB he :=
 encodable.choose_spec (existsu_fund_circ_of_basis hB he)
 
@@ -1188,14 +1099,14 @@ end encodable
 
 end of_indep
 
--- § 1.3
+/-! § 1.3. Rank. -/
 namespace of_indep
 
 variable {E}
 
 /-- def by Mario Carneiro https://leanprover.zulipchat.com/#narrow/stream/113489-new-members/subject/finset.20of.20subtype.20from.20filter/near/134578668 -/
 def indep_of_restriction (m : of_indep E) (X : finset E) : finset (finset {x : E // x ∈ X}) :=
-(m.indep).filter_map $ prestrict X
+m.indep.filter_map $ prestrict X
 -- def indep_of_restriction (m : indep E) (X : finset E) : finset (finset E) :=
 -- (m.indep).filter (λ I, I ⊆ X)
 
@@ -1247,8 +1158,8 @@ def restriction (m : of_indep E) (X : finset E) : of_indep {x : E // x ∈ X} :=
       exact this.symm ▸ he.2 },
     have H : insert e' x ∈ indep_of_restriction m X :=
       mem_restriction.mpr heinsert,
-    exact exists.intro e' ⟨heyx, H⟩,
-  end }
+    use e', exact ⟨heyx, H⟩,
+  end, }
 
 -- what about {x : E // x ∉ X} ?
 def deletion (m : of_indep E) (X : finset E) : of_indep {x : E // x ∈ univ \ X} :=
@@ -1286,8 +1197,8 @@ by { simp only [restriction, indep_of_restriction, mem_filter], exact ⟨hX, hXY
 X ∈ bases_bases_of_indep (m ¦ hY)-/
 
 lemma exists_basis_of_subset (X : finset E) (m : of_indep E) :
-  ∃ B, B ∈ (m ¦ X).bases_bases :=
-exists_mem_of_ne_empty $ B1 (m ¦ X)
+  ∃ B, B ∈ (m ¦ X).bases :=
+nonempty_of_ne_empty $ B1 (m ¦ X)
 
 /-lemma inter_of_span_of_subset_span {m : indep E} {X Y bX bY : finset α} {hXE : X ⊆ E}
   (hbX : spans bX hXE m) {hYE : Y ⊆ E} (hbY : spans bY hYE m) (hbXbY : bX ⊆ bY) : bY ∩ X = bX :=
